<?xml version="1.0"?>
<rdf:RDF xmlns="http://ontology.library.harvard.edu/geo/"
     xml:base="http://ontology.library.harvard.edu/geo/"
     xmlns:bf="http://id.loc.gov/ontologies/bibframe/"
     xmlns:bib="http://bibliotek-o.org/ontology/"
     xmlns:owl="http://www.w3.org/2002/07/owl#"
     xmlns:rdf="http://www.w3.org/1999/02/22-rdf-syntax-ns#"
     xmlns:xml="http://www.w3.org/XML/1998/namespace"
     xmlns:xsd="http://www.w3.org/2001/XMLSchema#"
     xmlns:foaf="http://xmlns.com/foaf/0.1#"
     xmlns:rdfs="http://www.w3.org/2000/01/rdf-schema#"
     xmlns:skos="http://www.w3.org/2004/02/skos/core#"
     xmlns:vann="http://purl.org/vocab/vann/"
     xmlns:dcterms="http://purl.org/dc/terms/">
    <owl:Ontology rdf:about="http://ontology.library.harvard.edu/geo/">
        <dcterms:issued>2018-03-26</dcterms:issued>
        <vann:preferredNamespacePrefix>gcro</vann:preferredNamespacePrefix>
        <rdfs:comment xml:lang="en">Geospatial and Cartographic Resources Ontology is an extension ontology of the bibliotek-o BIBFRAME 2.0 extension ontology produced by the Linked Data for Libraries Cartographic Materials project for use in describing geospatial and cartographic resources</rdfs:comment>
        <owl:versionInfo rdf:datatype="http://www.w3.org/2001/XMLSchema#string">Version 0.1</owl:versionInfo>
        <skos:definition xml:lang="en">Identifies the source for mathematical cartographic data,including scale, projection, and/or coordinates</skos:definition>
        <skos:prefLabel xml:lang="en">Cartographic data source</skos:prefLabel>
        <skos:prefLabel xml:lang="en">Geospatial and Cartographic Resources Ontology: extension ontology for describing cartographic materials</skos:prefLabel>
    </owl:Ontology>
    


    <!-- 
    ///////////////////////////////////////////////////////////////////////////////////////
    //
    // Annotation properties
    //
    ///////////////////////////////////////////////////////////////////////////////////////
     -->

    


    <!-- http://id.loc.gov/ontologies/bibframe/identifiedBy -->

    <owl:AnnotationProperty rdf:about="http://id.loc.gov/ontologies/bibframe/identifiedBy"/>
    


    <!-- http://id.loc.gov/ontologies/bibframe/identifies -->

    <owl:AnnotationProperty rdf:about="http://id.loc.gov/ontologies/bibframe/identifies"/>
    


    <!-- http://purl.org/dc/terms/issued -->

    <owl:AnnotationProperty rdf:about="http://purl.org/dc/terms/issued"/>
    


    <!-- http://purl.org/vocab/vann/preferredNamespacePrefix -->

    <owl:AnnotationProperty rdf:about="http://purl.org/vocab/vann/preferredNamespacePrefix"/>
    


    <!-- http://www.w3.org/1999/02/22-rdf-syntax-ns#value -->

    <owl:AnnotationProperty rdf:about="http://www.w3.org/1999/02/22-rdf-syntax-ns#value"/>
    


    <!-- http://www.w3.org/2002/07/owl#sameAs -->

    <owl:AnnotationProperty rdf:about="http://www.w3.org/2002/07/owl#sameAs"/>
    


    <!-- http://www.w3.org/2004/02/skos/core#altLabel -->

    <owl:AnnotationProperty rdf:about="http://www.w3.org/2004/02/skos/core#altLabel"/>
    


    <!-- http://www.w3.org/2004/02/skos/core#altfLabel -->

    <owl:AnnotationProperty rdf:about="http://www.w3.org/2004/02/skos/core#altfLabel"/>
    


    <!-- http://www.w3.org/2004/02/skos/core#definition -->

    <owl:AnnotationProperty rdf:about="http://www.w3.org/2004/02/skos/core#definition"/>
    


    <!-- http://www.w3.org/2004/02/skos/core#prefLabel -->

    <owl:AnnotationProperty rdf:about="http://www.w3.org/2004/02/skos/core#prefLabel"/>
    


    <!-- http://xmlns.com/foaf/0.1#page -->

    <owl:AnnotationProperty rdf:about="http://xmlns.com/foaf/0.1#page"/>
    


    <!-- 
    ///////////////////////////////////////////////////////////////////////////////////////
    //
    // Object Properties
    //
    ///////////////////////////////////////////////////////////////////////////////////////
     -->

    


    <!-- http://id.loc.gov/ontologies/bibframe/projection -->

    <owl:ObjectProperty rdf:about="http://id.loc.gov/ontologies/bibframe/projection">
        <owl:inverseOf rdf:resource="http://ontology.library.harvard.edu/geo/isProjectionOf"/>
    </owl:ObjectProperty>
    


    <!-- http://ontology.library.harvard.edu/geo/isGeometryOf -->

    <owl:ObjectProperty rdf:about="http://ontology.library.harvard.edu/geo/isGeometryOf">
        <owl:inverseOf rdf:resource="http://www.opengis.net/ont/geosparql#hasGeometry"/>
        <dcterms:issued>2018-03-26</dcterms:issued>
        <skos:prefLabel xml:lang="en">Is geometry of</skos:prefLabel>
    </owl:ObjectProperty>
    


    <!-- http://ontology.library.harvard.edu/geo/isProjectionOf -->

    <owl:ObjectProperty rdf:about="http://ontology.library.harvard.edu/geo/isProjectionOf">
        <dcterms:issued>2018-03-26</dcterms:issued>
        <skos:prefLabel xml:lang="en">Is projection of</skos:prefLabel>
    </owl:ObjectProperty>
    


    <!-- http://ontology.library.harvard.edu/geo/projectionPreservationProperty -->

    <owl:ObjectProperty rdf:about="http://ontology.library.harvard.edu/geo/projectionPreservationProperty">
        <rdfs:domain rdf:resource="http://id.loc.gov/ontologies/bibframe/Projection"/>
        <rdfs:range rdf:resource="http://ontology.library.harvard.edu/geo/ProjectionPreservationProperty"/>
        <dcterms:issued>2018-03-26</dcterms:issued>
        <skos:definition xml:lang="en">Geometric characteristic that the map projection attempts to preserve</skos:definition>
        <skos:prefLabel xml:lang="en">Has projection preservation property</skos:prefLabel>
    </owl:ObjectProperty>
    


    <!-- http://ontology.library.harvard.edu/geo/scaleAccuracy -->

    <owl:ObjectProperty rdf:about="http://ontology.library.harvard.edu/geo/scaleAccuracy">
        <rdfs:domain rdf:resource="http://id.loc.gov/ontologies/bibframe/Scale"/>
        <rdfs:range rdf:resource="http://ontology.library.harvard.edu/geo/ScaleAccuracy"/>
        <dcterms:issued>2018-03-26</dcterms:issued>
        <skos:definition xml:lang="en">Accuracy of the scale statement</skos:definition>
        <skos:prefLabel xml:lang="en">Has scale accuracy</skos:prefLabel>
    </owl:ObjectProperty>
    


    <!-- http://ontology.library.harvard.edu/geo/scaleSource -->

    <owl:ObjectProperty rdf:about="http://ontology.library.harvard.edu/geo/scaleSource">
        <rdfs:domain rdf:resource="http://id.loc.gov/ontologies/bibframe/Scale"/>
        <rdfs:range rdf:resource="http://ontology.library.harvard.edu/geo/ScaleSource"/>
        <dcterms:issued>2018-03-26</dcterms:issued>
        <skos:definition xml:lang="en">Has scale source</skos:definition>
        <skos:prefLabel xml:lang="en">Has scale source</skos:prefLabel>
    </owl:ObjectProperty>
    


    <!-- http://www.opengis.net/ont/geosparql#hasGeometry -->

    <owl:ObjectProperty rdf:about="http://www.opengis.net/ont/geosparql#hasGeometry"/>
    


    <!-- 
    ///////////////////////////////////////////////////////////////////////////////////////
    //
    // Data properties
    //
    ///////////////////////////////////////////////////////////////////////////////////////
     -->

    


    <!-- http://ontology.library.harvard.edu/geo/representativeFractionDenominator -->

    <owl:DatatypeProperty rdf:about="http://ontology.library.harvard.edu/geo/representativeFractionDenominator">
        <rdfs:domain rdf:resource="http://id.loc.gov/ontologies/bibframe/Scale"/>
        <rdfs:range rdf:resource="http://www.w3.org/2000/01/rdf-schema#Literal"/>
        <dcterms:issued>2018-03-26</dcterms:issued>
        <skos:definition xml:lang="en">The denominator of the scale&apos;s representative fraction</skos:definition>
        <skos:prefLabel xml:lang="en">Representative Fraction Denominator</skos:prefLabel>
    </owl:DatatypeProperty>
    


    <!-- 
    ///////////////////////////////////////////////////////////////////////////////////////
    //
    // Classes
    //
    ///////////////////////////////////////////////////////////////////////////////////////
     -->

    


    <!-- http://id.loc.gov/ontologies/bibframe/Cartography -->

    <owl:Class rdf:about="http://id.loc.gov/ontologies/bibframe/Cartography"/>
    


    <!-- http://id.loc.gov/ontologies/bibframe/Identifier -->

    <owl:Class rdf:about="http://id.loc.gov/ontologies/bibframe/Identifier"/>
    


    <!-- http://id.loc.gov/ontologies/bibframe/Projection -->

    <owl:Class rdf:about="http://id.loc.gov/ontologies/bibframe/Projection"/>
    


    <!-- http://id.loc.gov/ontologies/bibframe/Scale -->

    <owl:Class rdf:about="http://id.loc.gov/ontologies/bibframe/Scale"/>
    


    <!-- http://id.loc.gov/ontologies/bibframe/Source -->

    <owl:Class rdf:about="http://id.loc.gov/ontologies/bibframe/Source"/>
    


    <!-- http://ontology.library.harvard.edu/geo/ -->

    <owl:Class rdf:about="http://ontology.library.harvard.edu/geo/">
        <rdfs:subClassOf rdf:resource="http://id.loc.gov/ontologies/bibframe/Source"/>
    </owl:Class>
    


    <!-- http://ontology.library.harvard.edu/geo/AerialPhotographs -->

    <owl:Class rdf:about="http://ontology.library.harvard.edu/geo/AerialPhotographs">
        <rdfs:subClassOf rdf:resource="http://ontology.library.harvard.edu/geo/RemoteSensingImages"/>
        <dcterms:issued>2018-03-26</dcterms:issued>
        <skos:altLabel xml:lang="en">Photographs, Aerial</skos:altLabel>
        <skos:definition xml:lang="en"> Any photograph taken from the air. When used in a cartographic context, this term normally refers to photographs of the surface of the Earth (or other celestial body) taken downwards, vertically, or at a predetermined angle from the vertical (LCGFT)</skos:definition>
        <skos:prefLabel xml:lang="en">Aerial photographs</skos:prefLabel>
    </owl:Class>
    


    <!-- http://ontology.library.harvard.edu/geo/AerialViews -->

    <owl:Class rdf:about="http://ontology.library.harvard.edu/geo/AerialViews">
        <rdfs:subClassOf rdf:resource="http://ontology.library.harvard.edu/geo/CartographicViews"/>
        <dcterms:issued>2018-03-26</dcterms:issued>
        <skos:altLabel xml:lang="en">Bird&apos;s-eye views</skos:altLabel>
        <skos:altLabel xml:lang="en">Overhead views</skos:altLabel>
        <skos:altLabel xml:lang="en">Views, Aerial</skos:altLabel>
        <skos:altLabel xml:lang="en">Views, Bird&apos;s-eye</skos:altLabel>
        <skos:definition xml:lang="en">Representations of cities or landscapes portrayed as if viewed from above (LCGFT)</skos:definition>
        <skos:prefLabel xml:lang="en">Aerial views</skos:prefLabel>
    </owl:Class>
    


    <!-- http://ontology.library.harvard.edu/geo/AeronauticalCharts -->

    <owl:Class rdf:about="http://ontology.library.harvard.edu/geo/AeronauticalCharts">
        <rdfs:subClassOf rdf:resource="http://ontology.library.harvard.edu/geo/Maps"/>
        <dcterms:issued>2018-03-26</dcterms:issued>
        <skos:altLabel xml:lang="en">Navigational charts</skos:altLabel>
        <skos:definition xml:lang="en">Maps giving information intended for use in air navigation, such as compass rose, isogonic lines, location of landing fields, beacons, hazards to air navigation, etc. (LCGFT)</skos:definition>
        <skos:prefLabel xml:lang="en">Aeronautical charts</skos:prefLabel>
    </owl:Class>
    


    <!-- http://ontology.library.harvard.edu/geo/Aitoff -->

    <owl:Class rdf:about="http://ontology.library.harvard.edu/geo/Aitoff">
        <rdfs:subClassOf rdf:resource="http://ontology.library.harvard.edu/geo/AzimuthalProjection"/>
    </owl:Class>
    


    <!-- http://ontology.library.harvard.edu/geo/AlbersEqualArea -->

    <owl:Class rdf:about="http://ontology.library.harvard.edu/geo/AlbersEqualArea">
        <rdfs:subClassOf rdf:resource="http://ontology.library.harvard.edu/geo/ConicalProjection"/>
    </owl:Class>
    


    <!-- http://ontology.library.harvard.edu/geo/Armadillo -->

    <owl:Class rdf:about="http://ontology.library.harvard.edu/geo/Armadillo">
        <rdfs:subClassOf rdf:resource="http://ontology.library.harvard.edu/geo/UnclassifiedProjection"/>
    </owl:Class>
    


    <!-- http://ontology.library.harvard.edu/geo/AstronomicalModels -->

    <owl:Class rdf:about="http://ontology.library.harvard.edu/geo/AstronomicalModels">
        <rdfs:subClassOf rdf:resource="http://ontology.library.harvard.edu/geo/CartographicModels"/>
        <dcterms:issued>2018-03-26</dcterms:issued>
        <skos:altLabel xml:lang="en">Models, Astronomical</skos:altLabel>
        <skos:definition xml:lang="en">Astronomical models</skos:definition>
        <skos:prefLabel xml:lang="en">Astronomical models</skos:prefLabel>
    </owl:Class>
    


    <!-- http://ontology.library.harvard.edu/geo/Atlases -->

    <owl:Class rdf:about="http://ontology.library.harvard.edu/geo/Atlases">
        <rdfs:subClassOf rdf:resource="http://id.loc.gov/ontologies/bibframe/Cartography"/>
        <dcterms:issued>2018-03-26</dcterms:issued>
        <skos:altLabel xml:lang="en">Geographic atlases</skos:altLabel>
        <skos:altLabel xml:lang="en">Geographical atlases</skos:altLabel>
        <skos:definition xml:lang="en">A collection of maps designed to be kept (bound or loose) in a volume (LCGFT)</skos:definition>
        <skos:prefLabel xml:lang="en">Atlases</skos:prefLabel>
    </owl:Class>
    


    <!-- http://ontology.library.harvard.edu/geo/AzimuthalEquidistant -->

    <owl:Class rdf:about="http://ontology.library.harvard.edu/geo/AzimuthalEquidistant">
        <rdfs:subClassOf rdf:resource="http://ontology.library.harvard.edu/geo/AzimuthalProjection"/>
    </owl:Class>
    


    <!-- http://ontology.library.harvard.edu/geo/AzimuthalOther -->

    <owl:Class rdf:about="http://ontology.library.harvard.edu/geo/AzimuthalOther">
        <rdfs:subClassOf rdf:resource="http://ontology.library.harvard.edu/geo/AzimuthalProjection"/>
        <dcterms:issued>2018-03-26</dcterms:issued>
        <rdfs:comment xml:lang="en">MARC Map format projection code: az</rdfs:comment>
        <rdfs:comment>Type: Azimuthal</rdfs:comment>
        <skos:definition xml:lang="en">Azimuthal projection for which none of the other defined codes are appropriate</skos:definition>
        <skos:prefLabel xml:lang="en">Azimuthal, other</skos:prefLabel>
    </owl:Class>
    


    <!-- http://ontology.library.harvard.edu/geo/AzimuthalProjection -->

    <owl:Class rdf:about="http://ontology.library.harvard.edu/geo/AzimuthalProjection">
        <rdfs:subClassOf rdf:resource="http://id.loc.gov/ontologies/bibframe/Projection"/>
        <dcterms:issued>2018-03-26</dcterms:issued>
        <rdfs:comment xml:lang="en">MARC Map format projection code: a- (e.g. &quot;aa,&quot; etc.)</rdfs:comment>
        <skos:definition xml:lang="en">In standard presentation, azimuthal projections map meridians as straight lines and parallels as complete, concentric circles. They are radially symmetrical. In any presentation (or aspect), they preserve directions from the center point. This means great circles through the central point are represented by straight lines on the map (Wikipedia, List of Map Projections)</skos:definition>
        <skos:prefLabel xml:lang="en">Azimuthal projection</skos:prefLabel>
        <skos:prefLabel xml:lang="fr">projection azimutale</skos:prefLabel>
        <skos:prefLabel xml:lang="es">proyección acimutal</skos:prefLabel>
    </owl:Class>
    


    <!-- http://ontology.library.harvard.edu/geo/AzimuthalSpecificTypeUnknown -->

    <owl:Class rdf:about="http://ontology.library.harvard.edu/geo/AzimuthalSpecificTypeUnknown">
        <rdfs:subClassOf rdf:resource="http://ontology.library.harvard.edu/geo/AzimuthalProjection"/>
        <dcterms:issued>2018-03-26</dcterms:issued>
        <rdfs:comment xml:lang="en">MARC Map format projection code: au</rdfs:comment>
        <rdfs:comment>Type: Azimuthal</rdfs:comment>
        <skos:definition xml:lang="en">Only the projection type (azimuthal) is known, not the specific projection (MARC21). In standard presentation, azimuthal projections map meridians as straight lines and parallels as complete, concentric circles. They are radially symmetrical. In any presentation (or aspect), they preserve directions from the center point. This means great circles through the central point are represented by straight lines on the map (Wikipedia, List of Map Projections)</skos:definition>
        <skos:prefLabel xml:lang="en">Azimuthal, specific type unknown</skos:prefLabel>
    </owl:Class>
    


    <!-- http://ontology.library.harvard.edu/geo/BathymetricFormLines -->

    <owl:Class rdf:about="http://ontology.library.harvard.edu/geo/BathymetricFormLines">
        <rdfs:subClassOf rdf:resource="http://ontology.library.harvard.edu/geo/WaterRelief"/>
        <dcterms:issued>2018-03-26</dcterms:issued>
        <rdfs:comment xml:lang="en">MARC Map format relief code: f</rdfs:comment>
        <skos:definition xml:lang="en">Underwater relief shown by form lines (MARC21). These are also called formlines, which are lines, similar to contours, which depict the configuration of the underwater land without numerical indication of altitude (Adapted from Cartographic Resources Manual)</skos:definition>
        <skos:prefLabel xml:lang="en">Bathymetric form lines</skos:prefLabel>
    </owl:Class>
    


    <!-- http://ontology.library.harvard.edu/geo/BathymetricIsolines -->

    <owl:Class rdf:about="http://ontology.library.harvard.edu/geo/BathymetricIsolines">
        <rdfs:subClassOf rdf:resource="http://ontology.library.harvard.edu/geo/WaterRelief"/>
        <dcterms:issued>2018-03-26</dcterms:issued>
        <rdfs:comment xml:lang="en">MARC Map format relief code: k</rdfs:comment>
        <skos:definition xml:lang="en">Underwater relief (depth) shown by isolines (lines that represent constant depths) (MARC21)</skos:definition>
        <skos:prefLabel xml:lang="en">Bathymetric isolines</skos:prefLabel>
    </owl:Class>
    


    <!-- http://ontology.library.harvard.edu/geo/BathymetricSoundings -->

    <owl:Class rdf:about="http://ontology.library.harvard.edu/geo/BathymetricSoundings">
        <rdfs:subClassOf rdf:resource="http://ontology.library.harvard.edu/geo/WaterRelief"/>
        <dcterms:issued>2018-03-26</dcterms:issued>
        <rdfs:comment xml:lang="en">MARC Map format relief code: e</rdfs:comment>
        <skos:altLabel xml:lang="en">Bathymetry/soundings</skos:altLabel>
        <skos:altLabel xml:lang="en">Sounding</skos:altLabel>
        <skos:altLabel xml:lang="en">Soundings</skos:altLabel>
        <skos:definition xml:lang="en">Underwater depth shown by soundings (MARC21). A sounding is a measurement of the depth of water, usually expressed in feet or fathoms (Cartographic Materials)</skos:definition>
        <skos:prefLabel xml:lang="en">Bathymetric soundings</skos:prefLabel>
    </owl:Class>
    


    <!-- http://ontology.library.harvard.edu/geo/BathymetricTints -->

    <owl:Class rdf:about="http://ontology.library.harvard.edu/geo/BathymetricTints">
        <rdfs:subClassOf rdf:resource="http://ontology.library.harvard.edu/geo/WaterRelief"/>
        <dcterms:issued>2018-03-26</dcterms:issued>
        <rdfs:comment xml:lang="en">MARC Map format relief code: c</rdfs:comment>
        <skos:altLabel xml:lang="en">Hypsometric tints</skos:altLabel>
        <skos:definition xml:lang="en">Underwater relief shown by bathymetric tints (MARC21). Bathymetric tints are colors applied to the area between two selected contours where relief is depicted by a system of layers, specifically as applied to the depiction of water depth (DCRM-C)</skos:definition>
        <skos:prefLabel xml:lang="en">Bathymetric tints</skos:prefLabel>
    </owl:Class>
    


    <!-- http://ontology.library.harvard.edu/geo/Bonne -->

    <owl:Class rdf:about="http://ontology.library.harvard.edu/geo/Bonne">
        <rdfs:subClassOf rdf:resource="http://ontology.library.harvard.edu/geo/ConicalProjection"/>
        <rdfs:subClassOf rdf:resource="http://ontology.library.harvard.edu/geo/Cordiform"/>
    </owl:Class>
    


    <!-- http://ontology.library.harvard.edu/geo/BottleCharts -->

    <owl:Class rdf:about="http://ontology.library.harvard.edu/geo/BottleCharts">
        <rdfs:subClassOf rdf:resource="http://ontology.library.harvard.edu/geo/Maps"/>
        <dcterms:issued>2018-03-26</dcterms:issued>
        <skos:definition xml:lang="en">A chart of ocean surface currents to show the track of sealed bottles thrown from ships into the sea (LCGFT)</skos:definition>
        <skos:prefLabel xml:lang="en">Bottle-charts</skos:prefLabel>
    </owl:Class>
    


    <!-- http://ontology.library.harvard.edu/geo/Butterfly -->

    <owl:Class rdf:about="http://ontology.library.harvard.edu/geo/Butterfly">
        <rdfs:subClassOf rdf:resource="http://ontology.library.harvard.edu/geo/UnclassifiedProjection"/>
    </owl:Class>
    


    <!-- http://ontology.library.harvard.edu/geo/CadastralMaps -->

    <owl:Class rdf:about="http://ontology.library.harvard.edu/geo/CadastralMaps">
        <rdfs:subClassOf rdf:resource="http://ontology.library.harvard.edu/geo/Maps"/>
        <dcterms:issued>2018-03-26</dcterms:issued>
        <skos:altLabel xml:lang="en">Plan diagrams</skos:altLabel>
        <skos:altLabel xml:lang="en">Plan maps</skos:altLabel>
        <skos:altLabel xml:lang="en">Plat books</skos:altLabel>
        <skos:altLabel xml:lang="en">Plat diagrams</skos:altLabel>
        <skos:altLabel xml:lang="en">Plot diagrams</skos:altLabel>
        <skos:altLabel xml:lang="en">Plot maps</skos:altLabel>
        <skos:altLabel xml:lang="en">Property maps</skos:altLabel>
        <skos:altLabel xml:lang="en">Protraction maps</skos:altLabel>
        <skos:definition xml:lang="en">A map showing the boundaries of subdivisions of land, usually with the bearings and lengths thereof and the areas of individual tracts, for purposes of describing and recording ownership. A cadastral map may also show culture, drainage, and other features affecting the value and use of the land; also known as property map (LCGFT)</skos:definition>
        <skos:prefLabel xml:lang="en">Cadastral maps</skos:prefLabel>
    </owl:Class>
    


    <!-- http://ontology.library.harvard.edu/geo/CartSource -->

    <owl:Class rdf:about="http://ontology.library.harvard.edu/geo/CartSource"/>
    


    <!-- http://ontology.library.harvard.edu/geo/CartographicModels -->

    <owl:Class rdf:about="http://ontology.library.harvard.edu/geo/CartographicModels">
        <rdfs:subClassOf rdf:resource="http://id.loc.gov/ontologies/bibframe/Cartography"/>
        <dcterms:issued>2018-03-26</dcterms:issued>
        <skos:altLabel xml:lang="en">Models, Cartographic</skos:altLabel>
        <skos:definition xml:lang="en">A general category which denotes any three-dimensional representation of an object or geographic area, modeled in any size or medium [not including globes]</skos:definition>
        <skos:prefLabel xml:lang="en">Cartographic models</skos:prefLabel>
    </owl:Class>
    


    <!-- http://ontology.library.harvard.edu/geo/CartographicProfiles -->

    <owl:Class rdf:about="http://ontology.library.harvard.edu/geo/CartographicProfiles">
        <rdfs:subClassOf rdf:resource="http://id.loc.gov/ontologies/bibframe/Cartography"/>
        <dcterms:issued>2018-03-26</dcterms:issued>
        <skos:altLabel xml:lang="en">Profiles</skos:altLabel>
        <skos:altLabel xml:lang="en">Profiles, Cartographic</skos:altLabel>
        <skos:definition xml:lang="en">A scale representation of the intersection of a vertical surface (which may or may not be a plane) with the surface of the ground, or of the intersection of such a vertical surface with that of a conceptual three-dimensional model representing phenomena having a continuous distribution (e.g. rainfall).  The vertical scale is often exaggerated. (AACR2 mod.)</skos:definition>
        <skos:prefLabel xml:lang="en">Cartographic profiles</skos:prefLabel>
    </owl:Class>
    


    <!-- http://ontology.library.harvard.edu/geo/CartographicSections -->

    <owl:Class rdf:about="http://ontology.library.harvard.edu/geo/CartographicSections">
        <rdfs:subClassOf rdf:resource="http://id.loc.gov/ontologies/bibframe/Cartography"/>
        <dcterms:issued>2018-03-26</dcterms:issued>
        <skos:altLabel xml:lang="en">Sections, Cartographic</skos:altLabel>
        <skos:definition xml:lang="en">A scale representation of a vertical surface (commonly a plane) displaying both the profile where it intersects the surface of the ground, or some conceptual model, and the underlying structures along the plane of intersection (e.g. a geologic section) (AACR2 mod.)</skos:definition>
        <skos:prefLabel xml:lang="en">Cartographic sections</skos:prefLabel>
    </owl:Class>
    


    <!-- http://ontology.library.harvard.edu/geo/CartographicViews -->

    <owl:Class rdf:about="http://ontology.library.harvard.edu/geo/CartographicViews">
        <rdfs:subClassOf rdf:resource="http://id.loc.gov/ontologies/bibframe/Cartography"/>
        <dcterms:issued>2018-03-26</dcterms:issued>
        <skos:altLabel xml:lang="en">Views, Cartographic</skos:altLabel>
        <skos:definition xml:lang="en">A perspective representation of cities or landscapes</skos:definition>
        <skos:prefLabel xml:lang="en">Cartographic views</skos:prefLabel>
    </owl:Class>
    


    <!-- http://ontology.library.harvard.edu/geo/CassiniSoldner -->

    <owl:Class rdf:about="http://ontology.library.harvard.edu/geo/CassiniSoldner">
        <rdfs:subClassOf rdf:resource="http://ontology.library.harvard.edu/geo/CylindricalProjection"/>
    </owl:Class>
    


    <!-- http://ontology.library.harvard.edu/geo/CelestialCharts -->

    <owl:Class rdf:about="http://ontology.library.harvard.edu/geo/CelestialCharts">
        <rdfs:subClassOf rdf:resource="http://ontology.library.harvard.edu/geo/Maps"/>
        <dcterms:issued>2018-03-26</dcterms:issued>
        <skos:definition xml:lang="en">A map of representation of the celestial sphere, or of some part thereof (LCGFT)</skos:definition>
        <skos:prefLabel xml:lang="en">Celestial charts</skos:prefLabel>
    </owl:Class>
    


    <!-- http://ontology.library.harvard.edu/geo/CelestialGlobes -->

    <owl:Class rdf:about="http://ontology.library.harvard.edu/geo/CelestialGlobes">
        <rdfs:subClassOf rdf:resource="http://ontology.library.harvard.edu/geo/Globes"/>
        <dcterms:issued>2018-03-26</dcterms:issued>
        <skos:altLabel xml:lang="en">Globes, Celestial</skos:altLabel>
        <skos:definition xml:lang="en">A spherical representation of a celestial body, or the heavens</skos:definition>
        <skos:prefLabel xml:lang="en">Celestial globes</skos:prefLabel>
    </owl:Class>
    


    <!-- http://ontology.library.harvard.edu/geo/ChamberlinTrimetric -->

    <owl:Class rdf:about="http://ontology.library.harvard.edu/geo/ChamberlinTrimetric">
        <rdfs:subClassOf rdf:resource="http://ontology.library.harvard.edu/geo/AzimuthalProjection"/>
        <dcterms:issued>2018-03-26</dcterms:issued>
        <rdfs:comment xml:lang="en">MARC Map format projection code: an</rdfs:comment>
        <rdfs:comment>Type: Azimuthal</rdfs:comment>
        <skos:definition xml:lang="en">A map projection where three points are fixed on the globe and the points on the sphere are mapped onto a plane by triangulation. The Chamberlin trimetric projection is neither conformal nor equal-area. Rather, the projection was conceived to minimize distortion of distances everywhere with the side-effect of balancing between areal equivalence and conformality. This projection is not appropriate for mapping the entire sphere because the outer boundary would loop and overlap itself in most configurations (Wikipedia, Chamberlin Trimetric)</skos:definition>
        <skos:prefLabel xml:lang="en">Chamberlin trimetric</skos:prefLabel>
    </owl:Class>
    


    <!-- http://ontology.library.harvard.edu/geo/ComparativeMaps -->

    <owl:Class rdf:about="http://ontology.library.harvard.edu/geo/ComparativeMaps">
        <rdfs:subClassOf rdf:resource="http://ontology.library.harvard.edu/geo/Maps"/>
        <dcterms:issued>2018-03-26</dcterms:issued>
        <skos:altLabel xml:lang="en">Comparative area maps</skos:altLabel>
        <skos:definition xml:lang="en">A map comparing the relative size of two or more geographic areas</skos:definition>
        <skos:prefLabel xml:lang="en">Comparative maps</skos:prefLabel>
    </owl:Class>
    


    <!-- http://ontology.library.harvard.edu/geo/ConicOther -->

    <owl:Class rdf:about="http://ontology.library.harvard.edu/geo/ConicOther">
        <rdfs:subClassOf rdf:resource="http://ontology.library.harvard.edu/geo/ConicalProjection"/>
        <dcterms:issued>2018-03-26</dcterms:issued>
        <rdfs:comment xml:lang="en">MARC Map format projection code: cz</rdfs:comment>
        <skos:definition xml:lang="en">Conic projection for which none of the other defined codes are appropriate (MARC21)</skos:definition>
        <skos:prefLabel xml:lang="en">Conic, other</skos:prefLabel>
    </owl:Class>
    


    <!-- http://ontology.library.harvard.edu/geo/ConicSpecificTypeUnknown -->

    <owl:Class rdf:about="http://ontology.library.harvard.edu/geo/ConicSpecificTypeUnknown">
        <rdfs:subClassOf rdf:resource="http://ontology.library.harvard.edu/geo/ConicalProjection"/>
    </owl:Class>
    


    <!-- http://ontology.library.harvard.edu/geo/ConicalProjection -->

    <owl:Class rdf:about="http://ontology.library.harvard.edu/geo/ConicalProjection">
        <rdfs:subClassOf rdf:resource="http://id.loc.gov/ontologies/bibframe/Projection"/>
        <dcterms:issued>2018-03-26</dcterms:issued>
        <rdfs:comment xml:lang="en">MARC Map format projection code: c- (e.g. &quot;ca,&quot; etc.)</rdfs:comment>
        <skos:altLabel xml:lang="en">Conic projection</skos:altLabel>
        <skos:definition xml:lang="en">In standard presentation, conic (or conical) projections map meridians as straight lines, and parallels as arcs of circles (Wikipedia, List of Map Projections)</skos:definition>
        <skos:prefLabel xml:lang="en">Conical projection</skos:prefLabel>
        <skos:prefLabel xml:lang="fr">projection conique</skos:prefLabel>
        <skos:prefLabel xml:lang="es">proyección cónica</skos:prefLabel>
    </owl:Class>
    


    <!-- http://ontology.library.harvard.edu/geo/Contours -->

    <owl:Class rdf:about="http://ontology.library.harvard.edu/geo/Contours">
        <rdfs:subClassOf rdf:resource="http://ontology.library.harvard.edu/geo/LandRelief"/>
        <dcterms:issued>2018-03-26</dcterms:issued>
        <rdfs:comment xml:lang="en">MARC Map format relief code: a</rdfs:comment>
        <skos:altLabel xml:lang="en">Contour lines</skos:altLabel>
        <skos:definition xml:lang="en">Relief shown by contours (MARC21). A contour is a line joining points of equal vertical distance above or below a datum. Such a line on a map is a type of isoline (Cartographic Materials)</skos:definition>
        <skos:prefLabel xml:lang="en">Contours</skos:prefLabel>
    </owl:Class>
    


    <!-- http://ontology.library.harvard.edu/geo/Cordiform -->

    <owl:Class rdf:about="http://ontology.library.harvard.edu/geo/Cordiform">
        <rdfs:subClassOf rdf:resource="http://ontology.library.harvard.edu/geo/UnclassifiedProjection"/>
    </owl:Class>
    


    <!-- http://ontology.library.harvard.edu/geo/CylindricalOther -->

    <owl:Class rdf:about="http://ontology.library.harvard.edu/geo/CylindricalOther">
        <rdfs:subClassOf rdf:resource="http://ontology.library.harvard.edu/geo/CylindricalProjection"/>
        <dcterms:issued>2018-03-26</dcterms:issued>
        <rdfs:comment xml:lang="en">MARC Map format projection code: bz</rdfs:comment>
        <skos:definition xml:lang="en">Cylindrical projection for which none of the other defined codes are appropriate (MARC21)</skos:definition>
        <skos:prefLabel xml:lang="en">Cylindrical, other</skos:prefLabel>
    </owl:Class>
    


    <!-- http://ontology.library.harvard.edu/geo/CylindricalProjection -->

    <owl:Class rdf:about="http://ontology.library.harvard.edu/geo/CylindricalProjection">
        <rdfs:subClassOf rdf:resource="http://id.loc.gov/ontologies/bibframe/Projection"/>
        <dcterms:issued>2018-03-26</dcterms:issued>
        <rdfs:comment xml:lang="en">MARC Map format projection code: b- (e.g. &quot;ba,&quot; etc.)</rdfs:comment>
        <skos:definition xml:lang="en">In standard presentation, these map regularly-spaced meridians to equally spaced vertical lines, and parallels to horizontal lines (Wikipedia, List of Map Projections)</skos:definition>
        <skos:prefLabel xml:lang="en">Cylindrical projection</skos:prefLabel>
        <skos:prefLabel xml:lang="fr">projection cylindrique</skos:prefLabel>
        <skos:prefLabel xml:lang="es">proyección cilíndrica</skos:prefLabel>
    </owl:Class>
    


    <!-- http://ontology.library.harvard.edu/geo/CylindricalSpecificTypeUnknown -->

    <owl:Class rdf:about="http://ontology.library.harvard.edu/geo/CylindricalSpecificTypeUnknown">
        <rdfs:subClassOf rdf:resource="http://ontology.library.harvard.edu/geo/CylindricalProjection"/>
        <dcterms:issued>2018-03-26</dcterms:issued>
        <rdfs:comment xml:lang="en">MARC Map format projection code: bu</rdfs:comment>
        <skos:definition xml:lang="en">Only the projection type (cylindrical) is known, not the specific projection (MARC21). In standard presentation, these map regularly-spaced meridians to equally spaced vertical lines, and parallels to horizontal lines (Wikipedia, List of Map Projections). A map projection produced by projecting the geographic meridians and parallels onto a cylinder which is tangent to (or intersects) the surface of a sphere, and then developing the cylinder into a plane (Dict. of Mapping)</skos:definition>
        <skos:prefLabel xml:lang="en">Cylindrical, specific type unknown</skos:prefLabel>
    </owl:Class>
    


    <!-- http://ontology.library.harvard.edu/geo/DigitalCartographicResources -->

    <owl:Class rdf:about="http://ontology.library.harvard.edu/geo/DigitalCartographicResources">
        <rdfs:subClassOf rdf:resource="http://id.loc.gov/ontologies/bibframe/Cartography"/>
        <dcterms:issued>2018-03-26</dcterms:issued>
        <skos:definition xml:lang="en">Digital cartographic resource</skos:definition>
        <skos:prefLabel xml:lang="en">Digital cartographic resources</skos:prefLabel>
    </owl:Class>
    


    <!-- http://ontology.library.harvard.edu/geo/Dimaxion -->

    <owl:Class rdf:about="http://ontology.library.harvard.edu/geo/Dimaxion">
        <rdfs:subClassOf rdf:resource="http://ontology.library.harvard.edu/geo/UnclassifiedProjection"/>
    </owl:Class>
    


    <!-- http://ontology.library.harvard.edu/geo/EarlyMaps -->

    <owl:Class rdf:about="http://ontology.library.harvard.edu/geo/EarlyMaps">
        <rdfs:subClassOf rdf:resource="http://ontology.library.harvard.edu/geo/Maps"/>
        <dcterms:issued>2018-03-26</dcterms:issued>
        <skos:definition xml:lang="en">Generally refers to maps created before 1801</skos:definition>
        <skos:prefLabel xml:lang="en">Early maps</skos:prefLabel>
    </owl:Class>
    


    <!-- http://ontology.library.harvard.edu/geo/Eckert -->

    <owl:Class rdf:about="http://ontology.library.harvard.edu/geo/Eckert">
        <rdfs:subClassOf rdf:resource="http://ontology.library.harvard.edu/geo/UnclassifiedProjection"/>
    </owl:Class>
    


    <!-- http://ontology.library.harvard.edu/geo/Ephemerides -->

    <owl:Class rdf:about="http://ontology.library.harvard.edu/geo/Ephemerides">
        <rdfs:subClassOf rdf:resource="http://id.loc.gov/ontologies/bibframe/Cartography"/>
        <dcterms:issued>2018-03-26</dcterms:issued>
        <skos:definition xml:lang="en">Ephemeris plural ephemerides: a tabular statement of the assigned places of a celestial body for regular intervals. Table of the positions of celestial bodies at regular intervals, often with supplementary information. Constructed as early as the 4th century BC, ephemerides are still essential to astronomers and navigators. Modern ephemerides are calculated, with heavy computing and careful checking, after a mathematical description of a heavenly body&apos;s observed motion has been evolved. Various national ephemerides are published regularly; the U.S. ephemeris, first published in 1852, became the best and is now published jointly with the U.K. as The Astronomical Almanac (LCGFT)</skos:definition>
        <skos:prefLabel xml:lang="en">Ephemerides</skos:prefLabel>
    </owl:Class>
    


    <!-- http://ontology.library.harvard.edu/geo/EpsgCode -->

    <owl:Class rdf:about="http://ontology.library.harvard.edu/geo/EpsgCode">
        <rdfs:subClassOf rdf:resource="http://id.loc.gov/ontologies/bibframe/Identifier"/>
        <dcterms:issued>2018-03-26</dcterms:issued>
        <skos:definition xml:lang="en">EPSG Dataset Code</skos:definition>
        <skos:prefLabel xml:lang="en">EPSG Code</skos:prefLabel>
    </owl:Class>
    


    <!-- http://ontology.library.harvard.edu/geo/EquidistantConic -->

    <owl:Class rdf:about="http://ontology.library.harvard.edu/geo/EquidistantConic">
        <rdfs:subClassOf rdf:resource="http://ontology.library.harvard.edu/geo/ConicalProjection"/>
    </owl:Class>
    


    <!-- http://ontology.library.harvard.edu/geo/Equirectangular -->

    <owl:Class rdf:about="http://ontology.library.harvard.edu/geo/Equirectangular">
        <rdfs:subClassOf rdf:resource="http://ontology.library.harvard.edu/geo/CylindricalProjection"/>
    </owl:Class>
    


    <!-- http://ontology.library.harvard.edu/geo/EthnographicMaps -->

    <owl:Class rdf:about="http://ontology.library.harvard.edu/geo/EthnographicMaps">
        <rdfs:subClassOf rdf:resource="http://ontology.library.harvard.edu/geo/Maps"/>
        <dcterms:issued>2018-03-26</dcterms:issued>
        <skos:altLabel xml:lang="en">Anthropological maps</skos:altLabel>
        <skos:altLabel xml:lang="en">Ethnographical maps</skos:altLabel>
        <skos:altLabel xml:lang="en">Ethnological maps</skos:altLabel>
        <skos:definition xml:lang="en">Maps relating to ethnology, anthropology, and the diversity of humanity and human culture in general (Wikimedia Commons mod.)</skos:definition>
        <skos:prefLabel xml:lang="en">Ethnographic maps</skos:prefLabel>
    </owl:Class>
    


    <!-- http://ontology.library.harvard.edu/geo/FireInsuranceMaps -->

    <owl:Class rdf:about="http://ontology.library.harvard.edu/geo/FireInsuranceMaps">
        <rdfs:subClassOf rdf:resource="http://ontology.library.harvard.edu/geo/Maps"/>
        <dcterms:issued>2018-03-26</dcterms:issued>
        <skos:altLabel xml:lang="en">Fire insurance risk maps</skos:altLabel>
        <skos:altLabel xml:lang="en">Risk maps, Fire insurance</skos:altLabel>
        <skos:altLabel xml:lang="en">Sanborn fire insurance maps</skos:altLabel>
        <skos:altLabel xml:lang="en">Sanborn maps</skos:altLabel>
        <skos:definition xml:lang="en">Maps intended for use in calculating fire insurance risks prepared primarily for the use of fire insurance underwriters, which show detailed, accurate, and up-to-date information on potential fire hazards and risks for individual residences and commercial and industrial installations in urban and suburban areas.  Information shown includes the type of interior and exterior construction material, dimensions, and heights of buildings, block, lot and building numbers, occupancy of buildings, and such fire protection facilities as watermains, fire hydrants, and fire alarm boxes (LCGFT)</skos:definition>
        <skos:prefLabel xml:lang="en">Fire insurance maps</skos:prefLabel>
    </owl:Class>
    


    <!-- http://ontology.library.harvard.edu/geo/FlowMaps -->

    <owl:Class rdf:about="http://ontology.library.harvard.edu/geo/FlowMaps">
        <rdfs:subClassOf rdf:resource="http://ontology.library.harvard.edu/geo/Maps"/>
        <dcterms:issued>2018-03-26</dcterms:issued>
        <skos:altLabel xml:lang="en">Cartograms, Linear</skos:altLabel>
        <skos:altLabel xml:lang="en">Dynamic maps</skos:altLabel>
        <skos:altLabel xml:lang="en">Flow line maps</skos:altLabel>
        <skos:altLabel xml:lang="en">Line maps, Flow</skos:altLabel>
        <skos:altLabel xml:lang="en">Linear cartograms</skos:altLabel>
        <skos:definition xml:lang="en">Flow maps in cartography are by definition of Phan (2005) &quot;a mix of maps and flow charts, that show the movement of objects from one location to another, such as the number of people in a migration, the amount of goods being traded, or the number of packets in a network.&quot; Flow maps according to Harris (1999) &quot;can be used to show movement of almost anything, including tangible things such as people, products, natural resources, weather, etc, as well as intangible things such as know-how, talent, credit of goodwill&quot; (LCGFT)</skos:definition>
        <skos:prefLabel xml:lang="en">Flow maps</skos:prefLabel>
    </owl:Class>
    


    <!-- http://ontology.library.harvard.edu/geo/FormLines -->

    <owl:Class rdf:about="http://ontology.library.harvard.edu/geo/FormLines">
        <rdfs:subClassOf rdf:resource="http://ontology.library.harvard.edu/geo/LandRelief"/>
        <dcterms:issued>2018-03-26</dcterms:issued>
        <rdfs:comment xml:lang="en">MARC Map format relief code: f</rdfs:comment>
        <skos:altLabel xml:lang="en">Formlines</skos:altLabel>
        <skos:definition xml:lang="en">Land relief shown by form lines (MARC21). Form lines, also called formlines, are lines, similar to contours, which depict the configuration of the ground without numerical indication of altitude (Cartographic Resources Manual)</skos:definition>
        <skos:prefLabel xml:lang="en">Form lines</skos:prefLabel>
    </owl:Class>
    


    <!-- http://ontology.library.harvard.edu/geo/Gall -->

    <owl:Class rdf:about="http://ontology.library.harvard.edu/geo/Gall">
        <rdfs:subClassOf rdf:resource="http://ontology.library.harvard.edu/geo/CylindricalProjection"/>
    </owl:Class>
    


    <!-- http://ontology.library.harvard.edu/geo/GallPeters -->

    <owl:Class rdf:about="http://ontology.library.harvard.edu/geo/GallPeters">
        <rdfs:subClassOf rdf:resource="http://ontology.library.harvard.edu/geo/CylindricalProjection"/>
    </owl:Class>
    


    <!-- http://ontology.library.harvard.edu/geo/GaussKruger -->

    <owl:Class rdf:about="http://ontology.library.harvard.edu/geo/GaussKruger">
        <rdfs:subClassOf rdf:resource="http://ontology.library.harvard.edu/geo/CylindricalProjection"/>
    </owl:Class>
    


    <!-- http://ontology.library.harvard.edu/geo/Gazetteers -->

    <owl:Class rdf:about="http://ontology.library.harvard.edu/geo/Gazetteers">
        <rdfs:subClassOf rdf:resource="http://id.loc.gov/ontologies/bibframe/Cartography"/>
        <dcterms:issued>2018-03-26</dcterms:issued>
        <skos:altLabel xml:lang="en">Dictionaries, Geographical (Gazetteers)</skos:altLabel>
        <skos:altLabel xml:lang="en">Geographic dictionaries (Gazetteers)</skos:altLabel>
        <skos:altLabel xml:lang="en">Geographic indexes (Gazetteers)</skos:altLabel>
        <skos:altLabel xml:lang="en">Geographical dictionaries (Gazetteers)</skos:altLabel>
        <skos:altLabel xml:lang="en">Geographical indexes (Gazetteers)</skos:altLabel>
        <skos:altLabel xml:lang="en">Indexes, Geographical (Gazetteers)</skos:altLabel>
        <skos:definition xml:lang="en">A gazetteer is a geographical dictionary or directory, an important reference for information about places and place names, used in conjunction with a map or a full atlas. It typically contains information concerning the geographical makeup of a country, region, or continent as well as the social statistics and physical features, such as mountains, waterways, or roads (LCGFT)</skos:definition>
        <skos:prefLabel xml:lang="en">Gazetteers</skos:prefLabel>
    </owl:Class>
    


    <!-- http://ontology.library.harvard.edu/geo/GeneralVerticalNearSided -->

    <owl:Class rdf:about="http://ontology.library.harvard.edu/geo/GeneralVerticalNearSided">
        <rdfs:subClassOf rdf:resource="http://ontology.library.harvard.edu/geo/AzimuthalProjection"/>
        <dcterms:issued>2018-03-26</dcterms:issued>
        <rdfs:comment xml:lang="en">MARC Map format projection code: ag</rdfs:comment>
        <rdfs:comment>Type: Azimuthal</rdfs:comment>
        <skos:definition xml:lang="en">General vertical near-sided</skos:definition>
        <skos:prefLabel xml:lang="en">General vertical near-sided</skos:prefLabel>
    </owl:Class>
    


    <!-- http://ontology.library.harvard.edu/geo/GeologicalCrossSections -->

    <owl:Class rdf:about="http://ontology.library.harvard.edu/geo/GeologicalCrossSections">
        <rdfs:subClassOf rdf:resource="http://ontology.library.harvard.edu/geo/CartographicSections"/>
        <dcterms:issued>2018-03-26</dcterms:issued>
        <skos:altLabel xml:lang="en">Cross-sections, Geological</skos:altLabel>
        <skos:altLabel xml:lang="en">Geological cross-sections</skos:altLabel>
        <skos:definition xml:lang="en">A diagram or drawing that shows features transected by a given plane; specif. a vertical section drawn at right angles to the longer axis of a geologic feature, such as as the trend of an orebody, the mean direction of flow of a stream, or the axis of a fossil (LCGFT)</skos:definition>
        <skos:prefLabel xml:lang="en">Geological cross-sections</skos:prefLabel>
    </owl:Class>
    


    <!-- http://ontology.library.harvard.edu/geo/GeologicalMaps -->

    <owl:Class rdf:about="http://ontology.library.harvard.edu/geo/GeologicalMaps">
        <rdfs:subClassOf rdf:resource="http://ontology.library.harvard.edu/geo/Maps"/>
        <dcterms:issued>2018-03-26</dcterms:issued>
        <skos:altLabel xml:lang="en">Geologic maps</skos:altLabel>
        <skos:altLabel xml:lang="en">Geology maps</skos:altLabel>
        <skos:definition xml:lang="en">A map showing the structure and composition of the earth&apos;s crust (LCGFT)</skos:definition>
        <skos:prefLabel xml:lang="en">Geological maps</skos:prefLabel>
    </owl:Class>
    


    <!-- http://ontology.library.harvard.edu/geo/GeoreferencedCartographicResources -->

    <owl:Class rdf:about="http://ontology.library.harvard.edu/geo/GeoreferencedCartographicResources">
        <rdfs:subClassOf rdf:resource="http://ontology.library.harvard.edu/geo/GeospatialDigitalData"/>
        <dcterms:issued>2018-03-26</dcterms:issued>
        <skos:definition xml:lang="en">A scanned, paper map or cartographic resource that has been fit to real world coordinates using a GIS and is enabled for spatial display in a digital environment</skos:definition>
        <skos:prefLabel xml:lang="en">Georeferenced cartographic resources</skos:prefLabel>
    </owl:Class>
    


    <!-- http://ontology.library.harvard.edu/geo/GeospatialDatabases -->

    <owl:Class rdf:about="http://ontology.library.harvard.edu/geo/GeospatialDatabases">
        <rdfs:subClassOf rdf:resource="http://ontology.library.harvard.edu/geo/GeospatialDigitalData"/>
        <dcterms:issued>2018-03-26</dcterms:issued>
        <skos:altLabel xml:lang="en">Digital geographical databases</skos:altLabel>
        <skos:altLabel xml:lang="en">GDBs (Geodatabases)</skos:altLabel>
        <skos:altLabel xml:lang="en">GIS databases</skos:altLabel>
        <skos:altLabel xml:lang="en">GIS geodatabases</skos:altLabel>
        <skos:altLabel xml:lang="en">Geographic databases</skos:altLabel>
        <skos:altLabel xml:lang="en">Geographic information databases</skos:altLabel>
        <skos:altLabel xml:lang="en">Geographic information system databases</skos:altLabel>
        <skos:altLabel xml:lang="en">Geographic information systems databases</skos:altLabel>
        <skos:altLabel xml:lang="en">Geographical databases</skos:altLabel>
        <skos:altLabel xml:lang="en">Geographical information system databases</skos:altLabel>
        <skos:altLabel xml:lang="en">Geographical information systems databases</skos:altLabel>
        <skos:definition xml:lang="en">A database with geospatial data</skos:definition>
        <skos:prefLabel xml:lang="en">Geospatial databases</skos:prefLabel>
    </owl:Class>
    


    <!-- http://ontology.library.harvard.edu/geo/GeospatialDigitalData -->

    <owl:Class rdf:about="http://ontology.library.harvard.edu/geo/GeospatialDigitalData">
        <rdfs:subClassOf rdf:resource="http://id.loc.gov/ontologies/bibframe/Cartography"/>
        <dcterms:issued>2018-03-26</dcterms:issued>
        <skos:definition xml:lang="en">Digital geospatial data</skos:definition>
        <skos:prefLabel xml:lang="en">Geospatial digital data</skos:prefLabel>
    </owl:Class>
    


    <!-- http://ontology.library.harvard.edu/geo/Globes -->

    <owl:Class rdf:about="http://ontology.library.harvard.edu/geo/Globes">
        <rdfs:subClassOf rdf:resource="http://id.loc.gov/ontologies/bibframe/Cartography"/>
        <dcterms:issued>2018-03-26</dcterms:issued>
        <skos:definition xml:lang="en">A spherical representation of the earth, a celestial body, or the heavens (LCGFT)</skos:definition>
        <skos:prefLabel xml:lang="en">Globes</skos:prefLabel>
    </owl:Class>
    


    <!-- http://ontology.library.harvard.edu/geo/Gnomonic -->

    <owl:Class rdf:about="http://ontology.library.harvard.edu/geo/Gnomonic">
        <rdfs:subClassOf rdf:resource="http://ontology.library.harvard.edu/geo/AzimuthalProjection"/>
    </owl:Class>
    


    <!-- http://ontology.library.harvard.edu/geo/GoodesHomolographic -->

    <owl:Class rdf:about="http://ontology.library.harvard.edu/geo/GoodesHomolographic">
        <rdfs:subClassOf rdf:resource="http://ontology.library.harvard.edu/geo/CylindricalProjection"/>
    </owl:Class>
    


    <!-- http://ontology.library.harvard.edu/geo/GoodesHomolosine -->

    <owl:Class rdf:about="http://ontology.library.harvard.edu/geo/GoodesHomolosine">
        <rdfs:subClassOf rdf:resource="http://ontology.library.harvard.edu/geo/UnclassifiedProjection"/>
    </owl:Class>
    


    <!-- http://ontology.library.harvard.edu/geo/GoresMaps -->

    <owl:Class rdf:about="http://ontology.library.harvard.edu/geo/GoresMaps">
        <rdfs:subClassOf rdf:resource="http://ontology.library.harvard.edu/geo/Maps"/>
        <dcterms:issued>2018-03-26</dcterms:issued>
        <skos:altLabel xml:lang="en">Globe gores</skos:altLabel>
        <skos:definition xml:lang="en">Triangular or lune-shaped segment that can be fitted to the surface of a sphere with little distortion or deformation (LCGFT)</skos:definition>
        <skos:prefLabel xml:lang="en">Gores (Maps)</skos:prefLabel>
    </owl:Class>
    


    <!-- http://ontology.library.harvard.edu/geo/GradientTints -->

    <owl:Class rdf:about="http://ontology.library.harvard.edu/geo/GradientTints">
        <rdfs:subClassOf rdf:resource="http://ontology.library.harvard.edu/geo/LandRelief"/>
        <dcterms:issued>2018-03-26</dcterms:issued>
        <rdfs:comment xml:lang="en">MARC Map format relief code: c</rdfs:comment>
        <skos:altLabel xml:lang="en">Altitude tints</skos:altLabel>
        <skos:altLabel xml:lang="en">Hypsometric tints</skos:altLabel>
        <skos:definition xml:lang="en">Relief shown by gradient tints (MARC21). Gradient tints, also known as hypsometric or altitude tints, are colors applied to the area between two selected contours when relief is depicted by a system of layers (Cartographic Resources Manual)</skos:definition>
        <skos:prefLabel xml:lang="en">Gradient tints</skos:prefLabel>
    </owl:Class>
    


    <!-- http://ontology.library.harvard.edu/geo/GravityAnomalyMaps -->

    <owl:Class rdf:about="http://ontology.library.harvard.edu/geo/GravityAnomalyMaps">
        <rdfs:subClassOf rdf:resource="http://ontology.library.harvard.edu/geo/Maps"/>
        <dcterms:issued>2018-03-26</dcterms:issued>
        <skos:altLabel xml:lang="en">Gravity maps</skos:altLabel>
        <skos:definition xml:lang="en">Gravity anomaly maps depict the difference between theoretical computed gravity values and observed gravity values for a region of the earth&apos;s crust (LCGFT)</skos:definition>
        <skos:prefLabel xml:lang="en">Gravity anomaly maps</skos:prefLabel>
    </owl:Class>
    


    <!-- http://ontology.library.harvard.edu/geo/Hachures -->

    <owl:Class rdf:about="http://ontology.library.harvard.edu/geo/Hachures">
        <rdfs:subClassOf rdf:resource="http://ontology.library.harvard.edu/geo/LandRelief"/>
        <dcterms:issued>2018-03-26</dcterms:issued>
        <rdfs:comment xml:lang="en">MARC Map format relief code: d</rdfs:comment>
        <skos:definition xml:lang="en">Relief shown by hachures (MARC21). Hachures are short lines which follow the direction of maximum slope (Cartographic Resources Manual)</skos:definition>
        <skos:prefLabel xml:lang="en">Hachures</skos:prefLabel>
    </owl:Class>
    


    <!-- http://ontology.library.harvard.edu/geo/HorizontalScale -->

    <owl:Class rdf:about="http://ontology.library.harvard.edu/geo/HorizontalScale">
        <rdfs:subClassOf rdf:resource="http://id.loc.gov/ontologies/bibframe/Scale"/>
        <dcterms:issued>2018-03-26</dcterms:issued>
        <skos:definition xml:lang="en">The ratio of distances on a map to the corresponding horizontal distance in nature (Ency. Dict. of Cart.)</skos:definition>
        <skos:prefLabel xml:lang="en">Horizontal scale</skos:prefLabel>
        <skos:prefLabel xml:lang="es">escala horizontal</skos:prefLabel>
        <skos:prefLabel xml:lang="fr">échelle des longueurs</skos:prefLabel>
    </owl:Class>
    


    <!-- http://ontology.library.harvard.edu/geo/IndexMaps -->

    <owl:Class rdf:about="http://ontology.library.harvard.edu/geo/IndexMaps">
        <rdfs:subClassOf rdf:resource="http://ontology.library.harvard.edu/geo/Maps"/>
        <dcterms:issued>2018-03-26</dcterms:issued>
        <skos:altLabel xml:lang="en">Key maps</skos:altLabel>
        <skos:definition xml:lang="en">A map showing where to find collections of related data such as other maps, aerial photographs, statistical data, or descriptions of terrain. Also called a key map Index maps may be used to show references to the origin, place of deposit, or filing or other identifying characteristics of such data (LCGFT)</skos:definition>
        <skos:prefLabel xml:lang="en">Index maps</skos:prefLabel>
    </owl:Class>
    


    <!-- http://ontology.library.harvard.edu/geo/InteractiveDigitalCartographicResources -->

    <owl:Class rdf:about="http://ontology.library.harvard.edu/geo/InteractiveDigitalCartographicResources">
        <rdfs:subClassOf rdf:resource="http://ontology.library.harvard.edu/geo/DigitalCartographicResources"/>
        <dcterms:issued>2018-03-26</dcterms:issued>
        <skos:definition xml:lang="en">Born-digital cartographic resource that is interactive</skos:definition>
        <skos:prefLabel xml:lang="en">Interactive digital cartographic resources</skos:prefLabel>
    </owl:Class>
    


    <!-- http://ontology.library.harvard.edu/geo/Krovak -->

    <owl:Class rdf:about="http://ontology.library.harvard.edu/geo/Krovak">
        <rdfs:subClassOf rdf:resource="http://ontology.library.harvard.edu/geo/ConicalProjection"/>
    </owl:Class>
    


    <!-- http://ontology.library.harvard.edu/geo/LambertsAzimuthalEqualArea -->

    <owl:Class rdf:about="http://ontology.library.harvard.edu/geo/LambertsAzimuthalEqualArea">
        <rdfs:subClassOf rdf:resource="http://ontology.library.harvard.edu/geo/AzimuthalProjection"/>
    </owl:Class>
    


    <!-- http://ontology.library.harvard.edu/geo/LambertsConformalConic -->

    <owl:Class rdf:about="http://ontology.library.harvard.edu/geo/LambertsConformalConic">
        <rdfs:subClassOf rdf:resource="http://ontology.library.harvard.edu/geo/ConicalProjection"/>
    </owl:Class>
    


    <!-- http://ontology.library.harvard.edu/geo/LambertsCylindricalEqualArea -->

    <owl:Class rdf:about="http://ontology.library.harvard.edu/geo/LambertsCylindricalEqualArea">
        <rdfs:subClassOf rdf:resource="http://ontology.library.harvard.edu/geo/CylindricalProjection"/>
    </owl:Class>
    


    <!-- http://ontology.library.harvard.edu/geo/LandForms -->

    <owl:Class rdf:about="http://ontology.library.harvard.edu/geo/LandForms">
        <rdfs:subClassOf rdf:resource="http://ontology.library.harvard.edu/geo/LandRelief"/>
        <dcterms:issued>2018-03-26</dcterms:issued>
        <rdfs:comment xml:lang="en">MARC Map format relief code: j</rdfs:comment>
        <skos:altLabel xml:lang="en">Landform drawings</skos:altLabel>
        <skos:definition xml:lang="en">Relief shown by land forms (MARC21). Land form drawings are a method of relief that shows landforms by the systematic application of a standardized set of simplified pictorial symbols that represent the appearances such forms would have if viewed obliquely from the air at an angle of about 45º (Cartographic Resources Manual)</skos:definition>
        <skos:prefLabel xml:lang="en">Land forms</skos:prefLabel>
    </owl:Class>
    


    <!-- http://ontology.library.harvard.edu/geo/LandRelief -->

    <owl:Class rdf:about="http://ontology.library.harvard.edu/geo/LandRelief">
        <rdfs:subClassOf rdf:resource="http://ontology.library.harvard.edu/geo/Relief"/>
        <dcterms:issued>2018-03-26</dcterms:issued>
        <skos:definition xml:lang="en">Inequalities of elevation and the configuration of land features on the surface of the Earth that may be represented on maps or charts by contours, hypsometric tints, shading, spot elevations, or hachures (Cartographic Materials)</skos:definition>
        <skos:prefLabel xml:lang="en">Land relief</skos:prefLabel>
    </owl:Class>
    


    <!-- http://ontology.library.harvard.edu/geo/ManuscriptMaps -->

    <owl:Class rdf:about="http://ontology.library.harvard.edu/geo/ManuscriptMaps">
        <rdfs:subClassOf rdf:resource="http://ontology.library.harvard.edu/geo/Maps"/>
        <dcterms:issued>2018-03-26</dcterms:issued>
        <skos:definition xml:lang="en">The original drawing of a map as compiled or constructed from various data such as ground surveys and photographs (LCGFT)</skos:definition>
        <skos:prefLabel xml:lang="en">Manuscript maps</skos:prefLabel>
    </owl:Class>
    


    <!-- http://ontology.library.harvard.edu/geo/MappaeMundi -->

    <owl:Class rdf:about="http://ontology.library.harvard.edu/geo/MappaeMundi">
        <rdfs:subClassOf rdf:resource="http://ontology.library.harvard.edu/geo/Maps"/>
        <dcterms:issued>2018-03-26</dcterms:issued>
        <skos:altLabel xml:lang="en">Mappa mundi</skos:altLabel>
        <skos:altLabel xml:lang="en">Mappamundi</skos:altLabel>
        <skos:definition xml:lang="en">Used for medieval (usually circular) world maps, made between the fall of the western Roman empire in the later years of the 5th century AD and the end of the 15th century (LCGFT)</skos:definition>
        <skos:prefLabel xml:lang="en">Mappae mundi</skos:prefLabel>
    </owl:Class>
    


    <!-- http://ontology.library.harvard.edu/geo/Maps -->

    <owl:Class rdf:about="http://ontology.library.harvard.edu/geo/Maps">
        <rdfs:subClassOf rdf:resource="http://id.loc.gov/ontologies/bibframe/Cartography"/>
        <dcterms:issued>2018-03-26</dcterms:issued>
        <skos:altLabel xml:lang="en">Charts (Cartography)</skos:altLabel>
        <skos:altLabel xml:lang="en">Plans (Maps)</skos:altLabel>
        <skos:definition xml:lang="en">A graphic representation, usually on a plane surface and at an established scale, of natural and manmade features on or under the surface of the earth or other planetary body. 
            The features are positioned as accurately as possible, usually relative to a coordinate reference system. Also, a graphic representation of a part or the whole of the celestial sphere) physical map (LCGFT)</skos:definition>
        <skos:prefLabel xml:lang="en">Maps</skos:prefLabel>
    </owl:Class>
    


    <!-- http://ontology.library.harvard.edu/geo/MentalMaps -->

    <owl:Class rdf:about="http://ontology.library.harvard.edu/geo/MentalMaps">
        <rdfs:subClassOf rdf:resource="http://ontology.library.harvard.edu/geo/Maps"/>
        <dcterms:issued>2018-03-26</dcterms:issued>
        <skos:definition xml:lang="en">A mental map can best be explained as a visual display, inside a person&apos;s head, showing where a person has traveled. A mental map shows what the person knows about the location and the uniqueness of a place. No mental map is alike. Every human has his or her own mental map (LCGFT)</skos:definition>
        <skos:prefLabel xml:lang="en">Mental maps</skos:prefLabel>
    </owl:Class>
    


    <!-- http://ontology.library.harvard.edu/geo/Mercator -->

    <owl:Class rdf:about="http://ontology.library.harvard.edu/geo/Mercator">
        <rdfs:subClassOf rdf:resource="http://ontology.library.harvard.edu/geo/CylindricalProjection"/>
    </owl:Class>
    


    <!-- http://ontology.library.harvard.edu/geo/MeteorologicalCharts -->

    <owl:Class rdf:about="http://ontology.library.harvard.edu/geo/MeteorologicalCharts">
        <rdfs:subClassOf rdf:resource="http://ontology.library.harvard.edu/geo/Maps"/>
        <dcterms:issued>2018-03-26</dcterms:issued>
        <skos:definition xml:lang="en">A chart giving information about the weather (LCGFT)</skos:definition>
        <skos:prefLabel xml:lang="en">Meteorological charts</skos:prefLabel>
    </owl:Class>
    


    <!-- http://ontology.library.harvard.edu/geo/MilitaryMaps -->

    <owl:Class rdf:about="http://ontology.library.harvard.edu/geo/MilitaryMaps">
        <rdfs:subClassOf rdf:resource="http://ontology.library.harvard.edu/geo/Maps"/>
        <dcterms:issued>2018-03-26</dcterms:issued>
        <skos:definition xml:lang="en">A map designed particularly for military use (LCGFT)</skos:definition>
        <skos:prefLabel xml:lang="en">Military maps</skos:prefLabel>
    </owl:Class>
    


    <!-- http://ontology.library.harvard.edu/geo/Miller -->

    <owl:Class rdf:about="http://ontology.library.harvard.edu/geo/Miller">
        <rdfs:subClassOf rdf:resource="http://ontology.library.harvard.edu/geo/CylindricalProjection"/>
    </owl:Class>
    


    <!-- http://ontology.library.harvard.edu/geo/MillersBipolarObliqueConformalConic -->

    <owl:Class rdf:about="http://ontology.library.harvard.edu/geo/MillersBipolarObliqueConformalConic">
        <rdfs:subClassOf rdf:resource="http://ontology.library.harvard.edu/geo/UnclassifiedProjection"/>
        <dcterms:issued>2018-03-26</dcterms:issued>
        <rdfs:comment xml:lang="en">MARC Map format projection code: de</rdfs:comment>
        <skos:definition xml:lang="en">Miller&apos;s bipolar oblique conformal conic</skos:definition>
        <skos:prefLabel xml:lang="en">Miller&apos;s bipolar oblique conformal conic</skos:prefLabel>
    </owl:Class>
    


    <!-- http://ontology.library.harvard.edu/geo/MineMaps -->

    <owl:Class rdf:about="http://ontology.library.harvard.edu/geo/MineMaps">
        <rdfs:subClassOf rdf:resource="http://ontology.library.harvard.edu/geo/Maps"/>
        <dcterms:issued>2018-03-26</dcterms:issued>
        <skos:definition xml:lang="en">Maps recording mining activity, either specific mines or broader areas of mining. Maps can be topographic or cross-sectional in nature</skos:definition>
        <skos:prefLabel xml:lang="en">Mine maps</skos:prefLabel>
    </owl:Class>
    


    <!-- http://ontology.library.harvard.edu/geo/MiniatureMaps -->

    <owl:Class rdf:about="http://ontology.library.harvard.edu/geo/MiniatureMaps">
        <rdfs:subClassOf rdf:resource="http://ontology.library.harvard.edu/geo/Maps"/>
        <dcterms:issued>2018-03-26</dcterms:issued>
        <skos:definition xml:lang="en">Generally, any map with a size of 150 square centimeters or less (MiniatureMaps.net mod.)</skos:definition>
        <skos:prefLabel xml:lang="en">Miniature maps</skos:prefLabel>
    </owl:Class>
    


    <!-- http://ontology.library.harvard.edu/geo/ModifiedStereographicForAlaska -->

    <owl:Class rdf:about="http://ontology.library.harvard.edu/geo/ModifiedStereographicForAlaska">
        <rdfs:subClassOf rdf:resource="http://ontology.library.harvard.edu/geo/AzimuthalProjection"/>
        <dcterms:issued>2018-03-26</dcterms:issued>
        <rdfs:comment xml:lang="en">MARC Map format projection code: am</rdfs:comment>
        <rdfs:comment>Type: Azimuthal</rdfs:comment>
        <skos:definition xml:lang="en">Modified stereographic for Alaska</skos:definition>
        <skos:prefLabel xml:lang="en">Modified stereographic for Alaska</skos:prefLabel>
    </owl:Class>
    


    <!-- http://ontology.library.harvard.edu/geo/Mollweide -->

    <owl:Class rdf:about="http://ontology.library.harvard.edu/geo/Mollweide">
        <rdfs:subClassOf rdf:resource="http://ontology.library.harvard.edu/geo/CylindricalProjection"/>
    </owl:Class>
    


    <!-- http://ontology.library.harvard.edu/geo/NauticalCharts -->

    <owl:Class rdf:about="http://ontology.library.harvard.edu/geo/NauticalCharts">
        <rdfs:subClassOf rdf:resource="http://ontology.library.harvard.edu/geo/Maps"/>
        <dcterms:issued>2018-03-26</dcterms:issued>
        <skos:altLabel xml:lang="en">Hydrographic charts</skos:altLabel>
        <skos:altLabel xml:lang="en">Navigation charts</skos:altLabel>
        <skos:altLabel xml:lang="en">Navigation maps</skos:altLabel>
        <skos:altLabel xml:lang="en">Pilot charts</skos:altLabel>
        <skos:definition xml:lang="en">A chart designed for use in navigating ships, boats, or other watercraft (LCGFT)</skos:definition>
        <skos:prefLabel xml:lang="en">Nautical charts</skos:prefLabel>
    </owl:Class>
    


    <!-- http://ontology.library.harvard.edu/geo/NoAttemptToCode -->

    <owl:Class rdf:about="http://ontology.library.harvard.edu/geo/NoAttemptToCode">
        <rdfs:subClassOf rdf:resource="http://ontology.library.harvard.edu/geo/Relief"/>
        <dcterms:issued>2018-03-26</dcterms:issued>
        <rdfs:comment xml:lang="en">MARC Map format relief code: ||||</rdfs:comment>
        <skos:definition xml:lang="en">Relief not determined</skos:definition>
        <skos:prefLabel xml:lang="en">No attempt to code</skos:prefLabel>
    </owl:Class>
    


    <!-- http://ontology.library.harvard.edu/geo/NoLandRelief -->

    <owl:Class rdf:about="http://ontology.library.harvard.edu/geo/NoLandRelief">
        <rdfs:subClassOf rdf:resource="http://ontology.library.harvard.edu/geo/NoRelief"/>
        <dcterms:issued>2018-03-26</dcterms:issued>
        <skos:definition xml:lang="en">No land relief shown</skos:definition>
        <skos:prefLabel xml:lang="en">No land relief</skos:prefLabel>
    </owl:Class>
    


    <!-- http://ontology.library.harvard.edu/geo/NoRelief -->

    <owl:Class rdf:about="http://ontology.library.harvard.edu/geo/NoRelief">
        <rdfs:subClassOf rdf:resource="http://ontology.library.harvard.edu/geo/Relief"/>
        <dcterms:issued>2018-03-26</dcterms:issued>
        <rdfs:comment xml:lang="en">MARC Map format relief code: #</rdfs:comment>
        <skos:definition xml:lang="en">No relief shown</skos:definition>
        <skos:prefLabel xml:lang="en">No relief shown</skos:prefLabel>
    </owl:Class>
    


    <!-- http://ontology.library.harvard.edu/geo/NoWaterRelief -->

    <owl:Class rdf:about="http://ontology.library.harvard.edu/geo/NoWaterRelief">
        <rdfs:subClassOf rdf:resource="http://ontology.library.harvard.edu/geo/NoRelief"/>
        <dcterms:issued>2018-03-26</dcterms:issued>
        <skos:definition xml:lang="en">No underwater relief shown</skos:definition>
        <skos:prefLabel xml:lang="en">No water relief</skos:prefLabel>
    </owl:Class>
    


    <!-- http://ontology.library.harvard.edu/geo/NotDrawnToScale -->

    <owl:Class rdf:about="http://ontology.library.harvard.edu/geo/NotDrawnToScale">
        <rdfs:subClassOf rdf:resource="http://id.loc.gov/ontologies/bibframe/Scale"/>
        <dcterms:issued>2018-03-26</dcterms:issued>
        <skos:definition xml:lang="en">Used to describe a cartographic resource when it is not drawn to scale</skos:definition>
        <skos:prefLabel xml:lang="en">Not drawn to scale</skos:prefLabel>
    </owl:Class>
    


    <!-- http://ontology.library.harvard.edu/geo/ObliqueMercator -->

    <owl:Class rdf:about="http://ontology.library.harvard.edu/geo/ObliqueMercator">
        <rdfs:subClassOf rdf:resource="http://ontology.library.harvard.edu/geo/CylindricalProjection"/>
    </owl:Class>
    


    <!-- http://ontology.library.harvard.edu/geo/Orthographic -->

    <owl:Class rdf:about="http://ontology.library.harvard.edu/geo/Orthographic">
        <rdfs:subClassOf rdf:resource="http://ontology.library.harvard.edu/geo/AzimuthalProjection"/>
    </owl:Class>
    


    <!-- http://ontology.library.harvard.edu/geo/OtherProjection -->

    <owl:Class rdf:about="http://ontology.library.harvard.edu/geo/OtherProjection">
        <rdfs:subClassOf rdf:resource="http://id.loc.gov/ontologies/bibframe/Projection"/>
        <dcterms:issued>2018-03-26</dcterms:issued>
        <rdfs:comment xml:lang="en">MARC Map format projection code: zz</rdfs:comment>
        <skos:definition xml:lang="en">None of the other named projections are appropriate (MARC 21)</skos:definition>
        <skos:prefLabel xml:lang="en">Other projection</skos:prefLabel>
    </owl:Class>
    


    <!-- http://ontology.library.harvard.edu/geo/OtherRelief -->

    <owl:Class rdf:about="http://ontology.library.harvard.edu/geo/OtherRelief">
        <rdfs:subClassOf rdf:resource="http://ontology.library.harvard.edu/geo/Relief"/>
        <dcterms:issued>2018-03-26</dcterms:issued>
        <rdfs:comment xml:lang="en">MARC Map format relief code: z</rdfs:comment>
        <skos:definition xml:lang="en">None of the other defined codes are appropriate</skos:definition>
        <skos:prefLabel xml:lang="en">Other relief</skos:prefLabel>
    </owl:Class>
    


    <!-- http://ontology.library.harvard.edu/geo/OutlineMaps -->

    <owl:Class rdf:about="http://ontology.library.harvard.edu/geo/OutlineMaps">
        <rdfs:subClassOf rdf:resource="http://ontology.library.harvard.edu/geo/Maps"/>
        <dcterms:issued>2018-03-26</dcterms:issued>
        <skos:altLabel xml:lang="en">Base maps</skos:altLabel>
        <skos:definition xml:lang="en">A map showing just enough geographic information to permit the correct placement of additional details.  Outline maps correspond to what were at one time known as base maps; they usually show only cast lines, principal rivers, major civil boundaries, and large cities.  As much space as possible is left for placing the particular details or data desired.  An outline map presents less detail than what is now known as a base map (LCGFT)</skos:definition>
        <skos:prefLabel xml:lang="en">Outline maps</skos:prefLabel>
    </owl:Class>
    


    <!-- http://ontology.library.harvard.edu/geo/Panoramas -->

    <owl:Class rdf:about="http://ontology.library.harvard.edu/geo/Panoramas">
        <rdfs:subClassOf rdf:resource="http://ontology.library.harvard.edu/geo/CartographicViews"/>
        <dcterms:issued>2018-03-26</dcterms:issued>
        <skos:definition xml:lang="en">A perspective representation of the landscape in which the detail is shown as if projected onto a vertical plane or onto the insides of a cylinder centered vertically on the observer (Ency. Dict. of Cart.)</skos:definition>
        <skos:prefLabel xml:lang="en">Panoramas</skos:prefLabel>
    </owl:Class>
    


    <!-- http://ontology.library.harvard.edu/geo/Photomaps -->

    <owl:Class rdf:about="http://ontology.library.harvard.edu/geo/Photomaps">
        <rdfs:subClassOf rdf:resource="http://ontology.library.harvard.edu/geo/Maps"/>
        <dcterms:issued>2018-03-26</dcterms:issued>
        <skos:altLabel xml:lang="en">Orthophoto maps</skos:altLabel>
        <skos:altLabel xml:lang="en">Orthophotomaps</skos:altLabel>
        <skos:altLabel xml:lang="en">Photo maps</skos:altLabel>
        <skos:altLabel xml:lang="en">Photographic maps</skos:altLabel>
        <skos:definition xml:lang="en">A map made from assembling photographs and adding appropriate information such as a reference system, grid, labels, scale, and so forth (LCGFT)</skos:definition>
        <skos:prefLabel xml:lang="en">Photomaps</skos:prefLabel>
    </owl:Class>
    


    <!-- http://ontology.library.harvard.edu/geo/PhysicalMaps -->

    <owl:Class rdf:about="http://ontology.library.harvard.edu/geo/PhysicalMaps">
        <rdfs:subClassOf rdf:resource="http://ontology.library.harvard.edu/geo/Maps"/>
        <dcterms:issued>2018-03-26</dcterms:issued>
        <skos:definition xml:lang="en">A map representing the surface of the land or the floor of the oceans. In addition to representing the relief, physical maps show some natural phenomena such as oceanic currents, swamps, sands and deserts. Man-made structures or vegetation are not shown (LCGFT)</skos:definition>
        <skos:prefLabel xml:lang="en">Physical maps</skos:prefLabel>
    </owl:Class>
    


    <!-- http://ontology.library.harvard.edu/geo/PictorialMaps -->

    <owl:Class rdf:about="http://ontology.library.harvard.edu/geo/PictorialMaps">
        <rdfs:subClassOf rdf:resource="http://ontology.library.harvard.edu/geo/Maps"/>
        <dcterms:issued>2018-03-26</dcterms:issued>
        <skos:definition xml:lang="en">Maps that depict a given territory with a more artistic rather than technical style, usually showing an area as if viewed from above at an oblique angle (Wikipedia, Pictorial Maps)</skos:definition>
        <skos:prefLabel xml:lang="en">Pictorial maps</skos:prefLabel>
    </owl:Class>
    


    <!-- http://ontology.library.harvard.edu/geo/Pictorially -->

    <owl:Class rdf:about="http://ontology.library.harvard.edu/geo/Pictorially">
        <rdfs:subClassOf rdf:resource="http://ontology.library.harvard.edu/geo/LandRelief"/>
        <dcterms:issued>2018-03-26</dcterms:issued>
        <rdfs:comment xml:lang="en">MARC Map format relief code: i</rdfs:comment>
        <skos:definition xml:lang="en">Land forms and other topographic features shown in the correct planimetric position by pictorial symbols representing their appearance from a high oblique view (MARC21). Pictorial relief is not truly physiographic but usually consists of generalized drawings of hills, mountains, and bluffs. It was widely used before 1800. (Cartographic Resources Manual)</skos:definition>
        <skos:prefLabel xml:lang="en">Pictorially</skos:prefLabel>
    </owl:Class>
    


    <!-- http://ontology.library.harvard.edu/geo/PolarStereographic -->

    <owl:Class rdf:about="http://ontology.library.harvard.edu/geo/PolarStereographic">
        <rdfs:subClassOf rdf:resource="http://ontology.library.harvard.edu/geo/AzimuthalProjection"/>
        <dcterms:issued>2018-03-26</dcterms:issued>
        <rdfs:comment xml:lang="en">MARC Map format projection code: ap</rdfs:comment>
        <rdfs:comment>Type: Azimuthal</rdfs:comment>
        <skos:altfLabel xml:lang="en">Universal polar stereographic (UPS)</skos:altfLabel>
        <skos:definition xml:lang="en">The universal polar stereographic (UPS) coordinate system is used in conjunction with the universal transverse Mercator (UTM) coordinate system to locate positions on the surface of the earth. Like the UTM coordinate system, the UPS coordinate system uses a metric-based cartesian grid laid out on a conformally projected surface (Wikipedia, List of Map Projections)</skos:definition>
        <skos:prefLabel xml:lang="en">Polar stereographic</skos:prefLabel>
    </owl:Class>
    


    <!-- http://ontology.library.harvard.edu/geo/Polyconic -->

    <owl:Class rdf:about="http://ontology.library.harvard.edu/geo/Polyconic">
        <rdfs:subClassOf rdf:resource="http://ontology.library.harvard.edu/geo/ConicalProjection"/>
    </owl:Class>
    


    <!-- http://ontology.library.harvard.edu/geo/PortolanCharts -->

    <owl:Class rdf:about="http://ontology.library.harvard.edu/geo/PortolanCharts">
        <rdfs:subClassOf rdf:resource="http://ontology.library.harvard.edu/geo/Maps"/>
        <dcterms:issued>2018-03-26</dcterms:issued>
        <skos:definition xml:lang="en">A class of early coastal charts capable of navigational use which feature a network of interconnected lines (usually termed rhumb lines); place names written inland at right angles to the coast; drawn in ink on one or more skins following established color conventions; with coastlines shown in a general fashion with bays and headlines exaggerated and navigational hazards marked with crosses and dots (LCGFT)</skos:definition>
        <skos:prefLabel xml:lang="en">Portolan charts</skos:prefLabel>
    </owl:Class>
    


    <!-- http://ontology.library.harvard.edu/geo/ProjNoAttemptToCode -->

    <owl:Class rdf:about="http://ontology.library.harvard.edu/geo/ProjNoAttemptToCode">
        <rdfs:subClassOf rdf:resource="http://id.loc.gov/ontologies/bibframe/Projection"/>
        <dcterms:issued>2018-03-26</dcterms:issued>
        <rdfs:comment xml:lang="en">MARC Map format projection code: ||</rdfs:comment>
        <skos:definition xml:lang="en">No attempt to assign a projection to the resource</skos:definition>
        <skos:prefLabel xml:lang="en">No attempt to code</skos:prefLabel>
    </owl:Class>
    


    <!-- http://ontology.library.harvard.edu/geo/ProjectionNotSpecified -->

    <owl:Class rdf:about="http://ontology.library.harvard.edu/geo/ProjectionNotSpecified">
        <rdfs:subClassOf rdf:resource="http://id.loc.gov/ontologies/bibframe/Projection"/>
        <dcterms:issued>2018-03-26</dcterms:issued>
        <rdfs:comment xml:lang="en">MARC Map format projection code: ##</rdfs:comment>
        <skos:definition xml:lang="en">Used for most globes (MARC 21)</skos:definition>
        <skos:prefLabel xml:lang="en">Projection not specified</skos:prefLabel>
    </owl:Class>
    


    <!-- http://ontology.library.harvard.edu/geo/ProjectionPreservationProperty -->

    <owl:Class rdf:about="http://ontology.library.harvard.edu/geo/ProjectionPreservationProperty">
        <dcterms:issued>2018-03-26</dcterms:issued>
        <skos:definition xml:lang="en">Geometric characteristic that the map projection attempts to preserve</skos:definition>
        <skos:prefLabel xml:lang="en">Projection preservation property</skos:prefLabel>
    </owl:Class>
    


    <!-- http://ontology.library.harvard.edu/geo/QuadrangleMaps -->

    <owl:Class rdf:about="http://ontology.library.harvard.edu/geo/QuadrangleMaps">
        <rdfs:subClassOf rdf:resource="http://ontology.library.harvard.edu/geo/Maps"/>
        <dcterms:issued>2018-03-26</dcterms:issued>
        <skos:altLabel xml:lang="en">Quad maps</skos:altLabel>
        <skos:altLabel xml:lang="en">Quadrangular maps</skos:altLabel>
        <skos:definition xml:lang="en">Maps that cover a rectangular or nearly rectangular region defined by four specified points (LCGFT)</skos:definition>
        <skos:prefLabel xml:lang="en">Quadrangle maps</skos:prefLabel>
    </owl:Class>
    


    <!-- http://ontology.library.harvard.edu/geo/RasterData -->

    <owl:Class rdf:about="http://ontology.library.harvard.edu/geo/RasterData">
        <rdfs:subClassOf rdf:resource="http://ontology.library.harvard.edu/geo/GeospatialDigitalData"/>
        <dcterms:issued>2018-03-26</dcterms:issued>
        <skos:altLabel xml:lang="en">Raster maps</skos:altLabel>
        <skos:definition xml:lang="en">Data that are based on a cellular grid structure composed of rows and columns (a raster). Each grid cell or pixel is referenced by an x, y coordinate and is stored as an identifier to which additional attributes may be attached. Groups of cells with the same value represent map features (LCGFT)</skos:definition>
        <skos:prefLabel xml:lang="en">Raster data</skos:prefLabel>
    </owl:Class>
    


    <!-- http://ontology.library.harvard.edu/geo/Relief -->

    <owl:Class rdf:about="http://ontology.library.harvard.edu/geo/Relief">
        <dcterms:issued>2018-03-26</dcterms:issued>
        <skos:definition xml:lang="en">Inequalities of elevation and the configuration of land features on the surface of the Earth that may be represented on maps or charts by contours, hypsometric tints, shading, spot elevations, or hachures (Cartographic Materials). Also encompasses the depiction or indication of underwater topography, or the depths and shapes of underwater terrain (NOAA)</skos:definition>
        <skos:prefLabel xml:lang="en">Relief</skos:prefLabel>
        <foaf:page>https://docs.google.com/document/d/1KLICRXvbcFQfkpLXaIhky0NHAzgq4Ian5B_393LuULo/edit?usp=sharing</foaf:page>
    </owl:Class>
    


    <!-- http://ontology.library.harvard.edu/geo/ReliefModels -->

    <owl:Class rdf:about="http://ontology.library.harvard.edu/geo/ReliefModels">
        <rdfs:subClassOf rdf:resource="http://ontology.library.harvard.edu/geo/CartographicModels"/>
        <dcterms:issued>2018-03-26</dcterms:issued>
        <skos:altLabel xml:lang="en">3-D topographic maps</skos:altLabel>
        <skos:altLabel xml:lang="en">3-D topographical maps</skos:altLabel>
        <skos:altLabel xml:lang="en">3D topographic maps</skos:altLabel>
        <skos:altLabel xml:lang="en">3D topographical maps</skos:altLabel>
        <skos:altLabel xml:lang="en">Raised relief models</skos:altLabel>
        <skos:altLabel xml:lang="en">Relief models, Raised</skos:altLabel>
        <skos:altLabel xml:lang="en">Terrain models</skos:altLabel>
        <skos:altLabel xml:lang="en">Three-dimensional topographic maps</skos:altLabel>
        <skos:altLabel xml:lang="en">Three-dimensional topographical maps</skos:altLabel>
        <skos:altLabel xml:lang="en">Topographic models</skos:altLabel>
        <skos:definition xml:lang="en">A map whose surface is shaped to represent the topography in a region. Also called a terrain model (LCGFT)</skos:definition>
        <skos:prefLabel xml:lang="en">Relief models</skos:prefLabel>
    </owl:Class>
    


    <!-- http://ontology.library.harvard.edu/geo/RemoteSensingImages -->

    <owl:Class rdf:about="http://ontology.library.harvard.edu/geo/RemoteSensingImages">
        <rdfs:subClassOf rdf:resource="http://id.loc.gov/ontologies/bibframe/Cartography"/>
        <dcterms:issued>2018-03-26</dcterms:issued>
        <skos:altLabel xml:lang="en">Images, Remote-sensing</skos:altLabel>
        <skos:altLabel xml:lang="en">Multispectral scanning images</skos:altLabel>
        <skos:altLabel xml:lang="en">SLAR images</skos:altLabel>
        <skos:altLabel xml:lang="en">Satellite images</skos:altLabel>
        <skos:altLabel xml:lang="en">Side-looking airborne radar images</skos:altLabel>
        <skos:definition xml:lang="en">Images of planetary surfaces created by means of reflected or emitted electromagnetic energy (LCGFT)</skos:definition>
        <skos:prefLabel xml:lang="en">Remote-sensing images</skos:prefLabel>
    </owl:Class>
    


    <!-- http://ontology.library.harvard.edu/geo/RemoteSensingMaps -->

    <owl:Class rdf:about="http://ontology.library.harvard.edu/geo/RemoteSensingMaps">
        <rdfs:subClassOf rdf:resource="http://ontology.library.harvard.edu/geo/Maps"/>
        <dcterms:issued>2018-03-26</dcterms:issued>
        <skos:definition xml:lang="en">High-resolution topographic, bathymetric, or habitat maps created using remote-sensing applications which generate images by means of reflected or emitted electromagnetic energy (SWML mod.)</skos:definition>
        <skos:prefLabel xml:lang="en">Remote-sensing maps</skos:prefLabel>
    </owl:Class>
    


    <!-- http://ontology.library.harvard.edu/geo/RoadMaps -->

    <owl:Class rdf:about="http://ontology.library.harvard.edu/geo/RoadMaps">
        <rdfs:subClassOf rdf:resource="http://ontology.library.harvard.edu/geo/Maps"/>
        <dcterms:issued>2018-03-26</dcterms:issued>
        <skos:altLabel xml:lang="en">Roadmaps</skos:altLabel>
        <skos:altLabel xml:lang="en">Street maps</skos:altLabel>
        <skos:definition xml:lang="en">A map, usually at medium or small scale, showing the roads in a region (LCGFT)</skos:definition>
        <skos:prefLabel xml:lang="en">Road maps</skos:prefLabel>
    </owl:Class>
    


    <!-- http://ontology.library.harvard.edu/geo/Robinson -->

    <owl:Class rdf:about="http://ontology.library.harvard.edu/geo/Robinson">
        <rdfs:subClassOf rdf:resource="http://ontology.library.harvard.edu/geo/CylindricalProjection"/>
    </owl:Class>
    


    <!-- http://ontology.library.harvard.edu/geo/RockDrawings -->

    <owl:Class rdf:about="http://ontology.library.harvard.edu/geo/RockDrawings">
        <rdfs:subClassOf rdf:resource="http://ontology.library.harvard.edu/geo/LandRelief"/>
        <dcterms:issued>2018-03-26</dcterms:issued>
        <rdfs:comment xml:lang="en">MARC Map format relief code: m</rdfs:comment>
        <skos:definition xml:lang="en">Relief shown by rock drawings (MARC21). Rock drawings are stylized representations of steep rock faces which cannot be portrayed by other methods of representing relief (Cartographic Resources Manual)</skos:definition>
        <skos:prefLabel xml:lang="en">Rock drawings</skos:prefLabel>
    </owl:Class>
    


    <!-- http://ontology.library.harvard.edu/geo/ScaleAccuracy -->

    <owl:Class rdf:about="http://ontology.library.harvard.edu/geo/ScaleAccuracy">
        <dcterms:issued>2018-03-26</dcterms:issued>
        <skos:definition xml:lang="en">Scale accuracy</skos:definition>
        <skos:prefLabel xml:lang="en">Scale accuracy</skos:prefLabel>
    </owl:Class>
    


    <!-- http://ontology.library.harvard.edu/geo/ScaleIndeterminable -->

    <owl:Class rdf:about="http://ontology.library.harvard.edu/geo/ScaleIndeterminable">
        <rdfs:subClassOf rdf:resource="http://id.loc.gov/ontologies/bibframe/Scale"/>
        <dcterms:issued>2018-03-26</dcterms:issued>
        <skos:definition xml:lang="en">Used to describe a cartographic resource when an effort to determine the scale of a resource is impossible, for example, when there is a bar scale but no units of measurement are given (Cartographic Resources Manual)</skos:definition>
        <skos:prefLabel xml:lang="en">Scale indeterminable</skos:prefLabel>
    </owl:Class>
    


    <!-- http://ontology.library.harvard.edu/geo/ScaleNotDetermined -->

    <owl:Class rdf:about="http://ontology.library.harvard.edu/geo/ScaleNotDetermined">
        <rdfs:subClassOf rdf:resource="http://id.loc.gov/ontologies/bibframe/Scale"/>
        <dcterms:issued>2018-03-26</dcterms:issued>
        <skos:definition xml:lang="en">Use when scale is represented verbally or graphically in the material, but cannot be expressed as a representative fraction, e.g., because of lack of legibility or with unfamiliar units of measure (DCRM-C)</skos:definition>
        <skos:prefLabel xml:lang="en">Scale not determined</skos:prefLabel>
    </owl:Class>
    


    <!-- http://ontology.library.harvard.edu/geo/ScaleNotGiven -->

    <owl:Class rdf:about="http://ontology.library.harvard.edu/geo/ScaleNotGiven">
        <rdfs:subClassOf rdf:resource="http://id.loc.gov/ontologies/bibframe/Scale"/>
        <dcterms:issued>2018-03-26</dcterms:issued>
        <skos:definition xml:lang="en">If no scale is found in the material (whether as a representative fraction, verbally, or graphically), give the statement &quot;Scale not given&quot; (DCRM-C)</skos:definition>
        <skos:prefLabel xml:lang="en">Scale not given</skos:prefLabel>
    </owl:Class>
    


    <!-- http://ontology.library.harvard.edu/geo/ScaleSource -->

    <owl:Class rdf:about="http://ontology.library.harvard.edu/geo/ScaleSource">
        <dcterms:issued>2018-03-26</dcterms:issued>
        <skos:definition xml:lang="en">Source of the map scale</skos:definition>
        <skos:prefLabel xml:lang="en">Scale source</skos:prefLabel>
    </owl:Class>
    


    <!-- http://ontology.library.harvard.edu/geo/ScaleVaries -->

    <owl:Class rdf:about="http://ontology.library.harvard.edu/geo/ScaleVaries">
        <rdfs:subClassOf rdf:resource="http://id.loc.gov/ontologies/bibframe/Scale"/>
        <dcterms:issued>2018-03-26</dcterms:issued>
        <skos:definition xml:lang="en">A scale designation for a resource whose scale is variable across the resource, when the range of values cannot be determined (RDA). Used to describe one map/diagram/plan, etc. that is drawn on a variable scale</skos:definition>
        <skos:prefLabel xml:lang="en">Scale varies</skos:prefLabel>
    </owl:Class>
    


    <!-- http://ontology.library.harvard.edu/geo/ScalesDiffer -->

    <owl:Class rdf:about="http://ontology.library.harvard.edu/geo/ScalesDiffer">
        <rdfs:subClassOf rdf:resource="http://id.loc.gov/ontologies/bibframe/Scale"/>
        <dcterms:issued>2018-03-26</dcterms:issued>
        <skos:definition xml:lang="en">Used to describe a cartographic resource in which the main maps, etc., are of more than one scale (Adapted from Cartographic Resources Manual)</skos:definition>
        <skos:prefLabel xml:lang="en">Scales differ</skos:prefLabel>
    </owl:Class>
    


    <!-- http://ontology.library.harvard.edu/geo/ScannedCartographicResources -->

    <owl:Class rdf:about="http://ontology.library.harvard.edu/geo/ScannedCartographicResources">
        <rdfs:subClassOf rdf:resource="http://ontology.library.harvard.edu/geo/DigitalCartographicResources"/>
        <dcterms:issued>2018-03-26</dcterms:issued>
        <skos:altLabel xml:lang="en">Scanned maps</skos:altLabel>
        <skos:definition xml:lang="en">An analog resources that has been scanned for digital viewing as a static/non-interactive image</skos:definition>
        <skos:prefLabel xml:lang="en">Scanned cartographic resources</skos:prefLabel>
    </owl:Class>
    


    <!-- http://ontology.library.harvard.edu/geo/Shading -->

    <owl:Class rdf:about="http://ontology.library.harvard.edu/geo/Shading">
        <rdfs:subClassOf rdf:resource="http://ontology.library.harvard.edu/geo/LandRelief"/>
        <dcterms:issued>2018-03-26</dcterms:issued>
        <rdfs:comment xml:lang="en">MARC Map format relief code: b</rdfs:comment>
        <skos:definition xml:lang="en">Relief shown by shading, generally of a single color (MARC21). Shading is a relief method that provides an apparent three-dimensional configuration of the terrain by the use of shadows (Cartographic Resources Manual)</skos:definition>
        <skos:prefLabel xml:lang="en">Shading</skos:prefLabel>
    </owl:Class>
    


    <!-- http://ontology.library.harvard.edu/geo/Sinusoidal -->

    <owl:Class rdf:about="http://ontology.library.harvard.edu/geo/Sinusoidal">
        <rdfs:subClassOf rdf:resource="http://ontology.library.harvard.edu/geo/CylindricalProjection"/>
    </owl:Class>
    


    <!-- http://ontology.library.harvard.edu/geo/SpaceObliqueMercator -->

    <owl:Class rdf:about="http://ontology.library.harvard.edu/geo/SpaceObliqueMercator">
        <rdfs:subClassOf rdf:resource="http://ontology.library.harvard.edu/geo/CylindricalProjection"/>
    </owl:Class>
    


    <!-- http://ontology.library.harvard.edu/geo/SpotHeights -->

    <owl:Class rdf:about="http://ontology.library.harvard.edu/geo/SpotHeights">
        <rdfs:subClassOf rdf:resource="http://ontology.library.harvard.edu/geo/LandRelief"/>
        <dcterms:issued>2018-03-26</dcterms:issued>
        <rdfs:comment xml:lang="en">MARC Map format relief code: g</rdfs:comment>
        <skos:definition xml:lang="en">Relief shown by spot heights (MARC21). Spot Heights are points on a cartographic resource which represent the position of an indicated altitude (Cartographic Resources Manual)</skos:definition>
        <skos:prefLabel xml:lang="en">Spot heights</skos:prefLabel>
    </owl:Class>
    


    <!-- http://ontology.library.harvard.edu/geo/StaticDigitalCartographicResources -->

    <owl:Class rdf:about="http://ontology.library.harvard.edu/geo/StaticDigitalCartographicResources">
        <rdfs:subClassOf rdf:resource="http://ontology.library.harvard.edu/geo/DigitalCartographicResources"/>
        <dcterms:issued>2018-03-26</dcterms:issued>
        <skos:definition xml:lang="en">Born-digital cartographic resource that is static</skos:definition>
        <skos:prefLabel xml:lang="en">Static digital cartographic resources</skos:prefLabel>
    </owl:Class>
    


    <!-- http://ontology.library.harvard.edu/geo/StatisticalMaps -->

    <owl:Class rdf:about="http://ontology.library.harvard.edu/geo/StatisticalMaps">
        <rdfs:subClassOf rdf:resource="http://ontology.library.harvard.edu/geo/Maps"/>
        <dcterms:issued>2018-03-26</dcterms:issued>
        <skos:altLabel xml:lang="en">Maps of residuals</skos:altLabel>
        <skos:altLabel xml:lang="en">Residuals, Maps of</skos:altLabel>
        <skos:definition xml:lang="en">A special type of map in which the variation in quantity of a factor such as rainfall, population, or crops in a geographic area is indicated; a dot map is one type (Free Dictionary)</skos:definition>
        <skos:prefLabel xml:lang="en">Statistical maps</skos:prefLabel>
    </owl:Class>
    


    <!-- http://ontology.library.harvard.edu/geo/Stereographic -->

    <owl:Class rdf:about="http://ontology.library.harvard.edu/geo/Stereographic">
        <rdfs:subClassOf rdf:resource="http://ontology.library.harvard.edu/geo/AzimuthalProjection"/>
    </owl:Class>
    


    <!-- http://ontology.library.harvard.edu/geo/StickCharts -->

    <owl:Class rdf:about="http://ontology.library.harvard.edu/geo/StickCharts">
        <rdfs:subClassOf rdf:resource="http://ontology.library.harvard.edu/geo/Maps"/>
        <dcterms:issued>2018-03-26</dcterms:issued>
        <skos:definition xml:lang="en">Charts made by Pacific Islanders generally made of narrow strips of the center ribs of palm fronds lashed together with cord made from locally grown fiber plants. The arrangements of the sticks indicates the pattern of swells and wave masses caused by winds, rather than of currents. The positions of islands are marked approximately by shells or coral (LCGFT)</skos:definition>
        <skos:prefLabel xml:lang="en">Stick charts</skos:prefLabel>
    </owl:Class>
    


    <!-- http://ontology.library.harvard.edu/geo/StripMaps -->

    <owl:Class rdf:about="http://ontology.library.harvard.edu/geo/StripMaps">
        <rdfs:subClassOf rdf:resource="http://ontology.library.harvard.edu/geo/Maps"/>
        <dcterms:issued>2018-03-26</dcterms:issued>
        <skos:definition xml:lang="en">A map (as for an aviator) showing only a narrow band of territory (as 500 miles long and ten miles wide (LCGFT)</skos:definition>
        <skos:prefLabel xml:lang="en">Strip naps</skos:prefLabel>
    </owl:Class>
    


    <!-- http://ontology.library.harvard.edu/geo/TerrestrialGlobes -->

    <owl:Class rdf:about="http://ontology.library.harvard.edu/geo/TerrestrialGlobes">
        <rdfs:subClassOf rdf:resource="http://ontology.library.harvard.edu/geo/Globes"/>
        <dcterms:issued>2018-03-26</dcterms:issued>
        <skos:altLabel xml:lang="en">Globes, Terrestrial</skos:altLabel>
        <skos:definition xml:lang="en">A spherical representation of the earth</skos:definition>
        <skos:prefLabel xml:lang="en">Terrestrial globes</skos:prefLabel>
    </owl:Class>
    


    <!-- http://ontology.library.harvard.edu/geo/ThematicMaps -->

    <owl:Class rdf:about="http://ontology.library.harvard.edu/geo/ThematicMaps">
        <rdfs:subClassOf rdf:resource="http://ontology.library.harvard.edu/geo/Maps"/>
        <dcterms:issued>2018-03-26</dcterms:issued>
        <skos:altLabel xml:lang="en">Chloropleth maps</skos:altLabel>
        <skos:altLabel xml:lang="en">Single-topic maps</skos:altLabel>
        <skos:altLabel xml:lang="en">Special-purpose maps</skos:altLabel>
        <skos:altLabel xml:lang="en">Topical maps</skos:altLabel>
        <skos:definition xml:lang="en">A map whose principal purpose is depicting information other than that about the Earth&apos;s physical surface. Also called a topical map. Among the kinds of information shown on thematic maps are density of population, kind or amount of crops grown, types of soil, amount of rainfall and administrative subdivisions (LCGFT)</skos:definition>
        <skos:prefLabel xml:lang="en">Thematic maps</skos:prefLabel>
    </owl:Class>
    


    <!-- http://ontology.library.harvard.edu/geo/TopographicMaps -->

    <owl:Class rdf:about="http://ontology.library.harvard.edu/geo/TopographicMaps">
        <rdfs:subClassOf rdf:resource="http://ontology.library.harvard.edu/geo/Maps"/>
        <dcterms:issued>2018-03-26</dcterms:issued>
        <skos:altLabel xml:lang="en">Hypsographic maps</skos:altLabel>
        <skos:altLabel xml:lang="en">Hypsometric maps</skos:altLabel>
        <skos:altLabel xml:lang="en">Relief maps</skos:altLabel>
        <skos:altLabel xml:lang="en">Topo maps</skos:altLabel>
        <skos:altLabel xml:lang="en">Topographical maps</skos:altLabel>
        <skos:definition xml:lang="en">A map showing the horizontal and vertical locations of the natural and man-made features represented. Also called a relief map. Uses numbered contour lines or comparable symbols to show mountains, valleys and plains; a map whose principle purpose is to portray and identify the natural and artificial features on the Earth&apos;s surface as faithfully as possible within the limitations imposed by scale (LCGFT)</skos:definition>
        <skos:prefLabel xml:lang="en">Topographic maps</skos:prefLabel>
    </owl:Class>
    


    <!-- http://ontology.library.harvard.edu/geo/TouristMaps -->

    <owl:Class rdf:about="http://ontology.library.harvard.edu/geo/TouristMaps">
        <rdfs:subClassOf rdf:resource="http://ontology.library.harvard.edu/geo/Maps"/>
        <dcterms:issued>2018-03-26</dcterms:issued>
        <skos:definition xml:lang="en">Maps designed for tourists (LCGFT)</skos:definition>
        <skos:prefLabel xml:lang="en">Tourist maps</skos:prefLabel>
    </owl:Class>
    


    <!-- http://ontology.library.harvard.edu/geo/TransverseMercator -->

    <owl:Class rdf:about="http://ontology.library.harvard.edu/geo/TransverseMercator">
        <rdfs:subClassOf rdf:resource="http://ontology.library.harvard.edu/geo/CylindricalProjection"/>
    </owl:Class>
    


    <!-- http://ontology.library.harvard.edu/geo/UnclassifiedProjection -->

    <owl:Class rdf:about="http://ontology.library.harvard.edu/geo/UnclassifiedProjection">
        <rdfs:subClassOf rdf:resource="http://id.loc.gov/ontologies/bibframe/Projection"/>
        <dcterms:issued>2018-03-26</dcterms:issued>
        <rdfs:comment xml:lang="en">MARC Map format projection code: d- (e.g. &quot;da,&quot; etc.)</rdfs:comment>
        <skos:definition xml:lang="en">Named projections that are not azimuthal, cylindrical, or conic</skos:definition>
        <skos:prefLabel xml:lang="en">Unclassified projection</skos:prefLabel>
    </owl:Class>
    


    <!-- http://ontology.library.harvard.edu/geo/UpsideDownMaps -->

    <owl:Class rdf:about="http://ontology.library.harvard.edu/geo/UpsideDownMaps">
        <rdfs:subClassOf rdf:resource="http://ontology.library.harvard.edu/geo/Maps"/>
        <dcterms:issued>2018-03-26</dcterms:issued>
        <skos:altLabel xml:lang="en">Reversed maps</skos:altLabel>
        <skos:altLabel xml:lang="en">South-up maps</skos:altLabel>
        <skos:altLabel xml:lang="en">Upsidedown maps</skos:altLabel>
        <skos:definition xml:lang="en">Maps in which the orientation has been reversed and south appears at the top (LCGFT)</skos:definition>
        <skos:prefLabel xml:lang="en">Upside-down maps</skos:prefLabel>
    </owl:Class>
    


    <!-- http://ontology.library.harvard.edu/geo/VanDerGrinten -->

    <owl:Class rdf:about="http://ontology.library.harvard.edu/geo/VanDerGrinten">
        <rdfs:subClassOf rdf:resource="http://ontology.library.harvard.edu/geo/UnclassifiedProjection"/>
    </owl:Class>
    


    <!-- http://ontology.library.harvard.edu/geo/VectorData -->

    <owl:Class rdf:about="http://ontology.library.harvard.edu/geo/VectorData">
        <rdfs:subClassOf rdf:resource="http://ontology.library.harvard.edu/geo/GeospatialDigitalData"/>
        <dcterms:issued>2018-03-26</dcterms:issued>
        <skos:altLabel xml:lang="en">Vector maps</skos:altLabel>
        <skos:definition xml:lang="en">A data structure used to represent linear geographic features. Features are made of ordered lists of x, y or x, y, z coordinates and are represented by points, lines, or polygons; points connect to become lines, and lines connect to become polygons. Attributes are associated with each feature (LCGFT)</skos:definition>
        <skos:prefLabel xml:lang="en">Vector data</skos:prefLabel>
    </owl:Class>
    


    <!-- http://ontology.library.harvard.edu/geo/VerticalScale -->

    <owl:Class rdf:about="http://ontology.library.harvard.edu/geo/VerticalScale">
        <rdfs:subClassOf rdf:resource="http://id.loc.gov/ontologies/bibframe/Scale"/>
        <dcterms:issued>2018-03-26</dcterms:issued>
        <skos:definition xml:lang="en">The ratio of vertical distances on Profiles, Sections, Block Diagrams or three-dimensional representations to the corresponding distances in nature (Ency. Dict. of Cart.)</skos:definition>
        <skos:prefLabel xml:lang="en">Vertical scale</skos:prefLabel>
        <skos:prefLabel xml:lang="es">escala vertical</skos:prefLabel>
        <skos:prefLabel xml:lang="fr">échelle des hauteurs</skos:prefLabel>
    </owl:Class>
    


    <!-- http://ontology.library.harvard.edu/geo/WallMaps -->

    <owl:Class rdf:about="http://ontology.library.harvard.edu/geo/WallMaps">
        <rdfs:subClassOf rdf:resource="http://ontology.library.harvard.edu/geo/Maps"/>
        <dcterms:issued>2018-03-26</dcterms:issued>
        <skos:definition xml:lang="en">A map designed to be mounted or displayed on a wall, generally has devices on map to assist in hanging (LCGFT)</skos:definition>
        <skos:prefLabel xml:lang="en">Wall maps</skos:prefLabel>
    </owl:Class>
    


    <!-- http://ontology.library.harvard.edu/geo/WaterRelief -->

    <owl:Class rdf:about="http://ontology.library.harvard.edu/geo/WaterRelief">
        <rdfs:subClassOf rdf:resource="http://ontology.library.harvard.edu/geo/Relief"/>
        <dcterms:issued>2018-03-26</dcterms:issued>
        <skos:definition xml:lang="en">The depiction or indication of underwater topography, or the depths and shapes of underwater terrain (NOAA)</skos:definition>
        <skos:prefLabel xml:lang="en">Water relief</skos:prefLabel>
    </owl:Class>
    


    <!-- http://ontology.library.harvard.edu/geo/WorldMaps -->

    <owl:Class rdf:about="http://ontology.library.harvard.edu/geo/WorldMaps">
        <rdfs:subClassOf rdf:resource="http://ontology.library.harvard.edu/geo/Maps"/>
        <dcterms:issued>2018-03-26</dcterms:issued>
        <skos:definition xml:lang="en">A world map is a map of most or all of the surface of the Earth. World maps form a distinctive category of maps due to the problem of projection. Maps by necessity distort the presentation of the earth&apos;s surface. These distortions reach extremes in a world map. The many ways of projecting the earth reflect diverse technical and aesthetic goals for world maps (Wikipedia, World Maps)</skos:definition>
        <skos:prefLabel xml:lang="en">World maps</skos:prefLabel>
    </owl:Class>
    


    <!-- http://ontology.library.harvard.edu/geo/WormsEyeViews -->

    <owl:Class rdf:about="http://ontology.library.harvard.edu/geo/WormsEyeViews">
        <rdfs:subClassOf rdf:resource="http://ontology.library.harvard.edu/geo/CartographicViews"/>
        <dcterms:issued>2018-03-26</dcterms:issued>
        <skos:altLabel xml:lang="en">Views, Worm&apos;s-eye</skos:altLabel>
        <skos:definition xml:lang="en">Representations of cities or landscapes portrayed as if viewed from a very low viewpoint (LCGFT)</skos:definition>
        <skos:prefLabel xml:lang="en">Worm&apos;s-eye views</skos:prefLabel>
    </owl:Class>
    


    <!-- http://ontology.library.harvard.edu/geo/ZoningMaps -->

    <owl:Class rdf:about="http://ontology.library.harvard.edu/geo/ZoningMaps">
        <rdfs:subClassOf rdf:resource="http://ontology.library.harvard.edu/geo/Maps"/>
        <dcterms:issued>2018-03-26</dcterms:issued>
        <skos:altLabel xml:lang="en">Zoning district maps</skos:altLabel>
        <skos:definition xml:lang="en">Zoning maps show the boundaries of zoning districts throughout the city (LCGFT)</skos:definition>
        <skos:prefLabel xml:lang="en">Zoning maps</skos:prefLabel>
    </owl:Class>
    


    <!-- 
    ///////////////////////////////////////////////////////////////////////////////////////
    //
    // Individuals
    //
    ///////////////////////////////////////////////////////////////////////////////////////
     -->

    


    <!-- http://ontology.library.harvard.edu/geo/Aitoff -->

    <owl:NamedIndividual rdf:about="http://ontology.library.harvard.edu/geo/Aitoff">
        <projectionPreservationProperty rdf:resource="http://ontology.library.harvard.edu/geo/Compromise"/>
    </owl:NamedIndividual>
    


    <!-- http://ontology.library.harvard.edu/geo/AlbersEqualArea -->

    <owl:NamedIndividual rdf:about="http://ontology.library.harvard.edu/geo/AlbersEqualArea">
        <projectionPreservationProperty rdf:resource="http://ontology.library.harvard.edu/geo/EqualArea"/>
    </owl:NamedIndividual>
    


    <!-- http://ontology.library.harvard.edu/geo/ApproximateScale -->

    <owl:NamedIndividual rdf:about="http://ontology.library.harvard.edu/geo/ApproximateScale">
        <rdf:type rdf:resource="http://ontology.library.harvard.edu/geo/ScaleAccuracy"/>
        <dcterms:issued>2018-03-26</dcterms:issued>
        <skos:definition xml:lang="en">Approximate scale of cartographic resource</skos:definition>
        <skos:prefLabel xml:lang="en">Approximate scale</skos:prefLabel>
    </owl:NamedIndividual>
    


    <!-- http://ontology.library.harvard.edu/geo/Armadillo -->

    <owl:NamedIndividual rdf:about="http://ontology.library.harvard.edu/geo/Armadillo">
        <projectionPreservationProperty rdf:resource="http://ontology.library.harvard.edu/geo/Compromise"/>
    </owl:NamedIndividual>
    


    <!-- http://ontology.library.harvard.edu/geo/AzimuthalEquidistant -->

    <owl:NamedIndividual rdf:about="http://ontology.library.harvard.edu/geo/AzimuthalEquidistant">
        <projectionPreservationProperty rdf:resource="http://ontology.library.harvard.edu/geo/Equidistant"/>
    </owl:NamedIndividual>
    


    <!-- http://ontology.library.harvard.edu/geo/Bonne -->

    <owl:NamedIndividual rdf:about="http://ontology.library.harvard.edu/geo/Bonne">
        <projectionPreservationProperty rdf:resource="http://ontology.library.harvard.edu/geo/EqualArea"/>
    </owl:NamedIndividual>
    


    <!-- http://ontology.library.harvard.edu/geo/Bound -->

    <owl:NamedIndividual rdf:about="http://ontology.library.harvard.edu/geo/Bound">
        <rdf:type rdf:resource="http://ontology.library.harvard.edu/geo/CartSource"/>
        <dcterms:issued>2018-03-26</dcterms:issued>
        <rdfs:comment xml:lang="en">MARC Cartographic Data Source Code: bound</rdfs:comment>
        <skos:definition xml:lang="en">The Klokan Technologies Bounding Box Tool</skos:definition>
        <skos:prefLabel xml:lang="en">Bounding Box (Klokan Technologies)</skos:prefLabel>
        <foaf:page>http://boundingbox.klokantech.com/</foaf:page>
    </owl:NamedIndividual>
    


    <!-- http://ontology.library.harvard.edu/geo/Butterfly -->

    <owl:NamedIndividual rdf:about="http://ontology.library.harvard.edu/geo/Butterfly">
        <projectionPreservationProperty rdf:resource="http://ontology.library.harvard.edu/geo/Compromise"/>
    </owl:NamedIndividual>
    


    <!-- http://ontology.library.harvard.edu/geo/CalculatedFromPrimarySource -->

    <owl:NamedIndividual rdf:about="http://ontology.library.harvard.edu/geo/CalculatedFromPrimarySource">
        <rdf:type rdf:resource="http://ontology.library.harvard.edu/geo/ScaleSource"/>
        <dcterms:issued>2018-03-26</dcterms:issued>
        <skos:definition xml:lang="en">Source of scale is calculated from the primary source</skos:definition>
        <skos:prefLabel xml:lang="en">Scale calculated</skos:prefLabel>
    </owl:NamedIndividual>
    


    <!-- http://ontology.library.harvard.edu/geo/CassiniSoldner -->

    <owl:NamedIndividual rdf:about="http://ontology.library.harvard.edu/geo/CassiniSoldner">
        <projectionPreservationProperty rdf:resource="http://ontology.library.harvard.edu/geo/Equidistant"/>
    </owl:NamedIndividual>
    


    <!-- http://ontology.library.harvard.edu/geo/Compromise -->

    <owl:NamedIndividual rdf:about="http://ontology.library.harvard.edu/geo/Compromise">
        <rdf:type rdf:resource="http://ontology.library.harvard.edu/geo/ProjectionPreservationProperty"/>
        <dcterms:issued>2018-03-26</dcterms:issued>
        <skos:definition xml:lang="en">Neither conformal nor equal-area, but a balance intended to reduce overall distortion (Wikipedia, List of Map Projections)</skos:definition>
        <skos:prefLabel xml:lang="en">Compromise map projection</skos:prefLabel>
    </owl:NamedIndividual>
    


    <!-- http://ontology.library.harvard.edu/geo/Conformal -->

    <owl:NamedIndividual rdf:about="http://ontology.library.harvard.edu/geo/Conformal">
        <rdf:type rdf:resource="http://ontology.library.harvard.edu/geo/ProjectionPreservationProperty"/>
        <dcterms:issued>2018-03-26</dcterms:issued>
        <skos:definition xml:lang="en">Preserves angles locally, implying that local shapes are not distorted (Wikipedia, List of Map Projections)</skos:definition>
        <skos:prefLabel xml:lang="en">Conformal map projection</skos:prefLabel>
    </owl:NamedIndividual>
    


    <!-- http://ontology.library.harvard.edu/geo/ConicSpecificTypeUnknown -->

    <owl:NamedIndividual rdf:about="http://ontology.library.harvard.edu/geo/ConicSpecificTypeUnknown">
        <projectionPreservationProperty rdf:resource="http://ontology.library.harvard.edu/geo/Compromise"/>
    </owl:NamedIndividual>
    


    <!-- http://ontology.library.harvard.edu/geo/Cordiform -->

    <owl:NamedIndividual rdf:about="http://ontology.library.harvard.edu/geo/Cordiform">
        <projectionPreservationProperty rdf:resource="http://ontology.library.harvard.edu/geo/EqualArea"/>
        <projectionPreservationProperty rdf:resource="http://ontology.library.harvard.edu/geo/Equidistant"/>
    </owl:NamedIndividual>
    


    <!-- http://ontology.library.harvard.edu/geo/DerivedOther -->

    <owl:NamedIndividual rdf:about="http://ontology.library.harvard.edu/geo/DerivedOther">
        <rdf:type rdf:resource="http://ontology.library.harvard.edu/geo/ScaleSource"/>
        <dcterms:issued>2018-03-26</dcterms:issued>
        <skos:definition xml:lang="en">Source of scale is derived from an external resource</skos:definition>
        <skos:prefLabel xml:lang="en">Scale derived</skos:prefLabel>
    </owl:NamedIndividual>
    


    <!-- http://ontology.library.harvard.edu/geo/Dimaxion -->

    <owl:NamedIndividual rdf:about="http://ontology.library.harvard.edu/geo/Dimaxion">
        <projectionPreservationProperty rdf:resource="http://ontology.library.harvard.edu/geo/Compromise"/>
    </owl:NamedIndividual>
    


    <!-- http://ontology.library.harvard.edu/geo/Eckert -->

    <owl:NamedIndividual rdf:about="http://ontology.library.harvard.edu/geo/Eckert">
        <projectionPreservationProperty rdf:resource="http://ontology.library.harvard.edu/geo/EqualArea"/>
    </owl:NamedIndividual>
    


    <!-- http://ontology.library.harvard.edu/geo/EpsgCode4326 -->

    <owl:NamedIndividual rdf:about="http://ontology.library.harvard.edu/geo/EpsgCode4326">
        <rdf:type rdf:resource="http://ontology.library.harvard.edu/geo/EpsgCode"/>
        <bf:identifies rdf:resource="http://ontology.library.harvard.edu/geo/ProjectionEpsg4326"/>
        <dcterms:issued>2018-03-26</dcterms:issued>
        <rdf:value>4326</rdf:value>
        <skos:definition xml:lang="en">World Geodetic System 1984</skos:definition>
        <skos:prefLabel xml:lang="en">WGS 84</skos:prefLabel>
        <foaf:page>http://epsg.io/4326</foaf:page>
    </owl:NamedIndividual>
    


    <!-- http://ontology.library.harvard.edu/geo/EqualArea -->

    <owl:NamedIndividual rdf:about="http://ontology.library.harvard.edu/geo/EqualArea">
        <rdf:type rdf:resource="http://ontology.library.harvard.edu/geo/ProjectionPreservationProperty"/>
        <dcterms:issued>2018-03-26</dcterms:issued>
        <skos:definition xml:lang="en">Areas are conserved (Wikipedia, List of Map Projections)</skos:definition>
        <skos:prefLabel xml:lang="en">Equal area map projection</skos:prefLabel>
    </owl:NamedIndividual>
    


    <!-- http://ontology.library.harvard.edu/geo/Equidistant -->

    <owl:NamedIndividual rdf:about="http://ontology.library.harvard.edu/geo/Equidistant">
        <rdf:type rdf:resource="http://ontology.library.harvard.edu/geo/ProjectionPreservationProperty"/>
        <dcterms:issued>2018-03-26</dcterms:issued>
        <skos:definition xml:lang="en">All distances from one (or two) points are correct. Other equidistant properties are mentioned in the notes (Wikipedia, List of Map Projections)</skos:definition>
        <skos:prefLabel xml:lang="en">Equidistant map projection</skos:prefLabel>
    </owl:NamedIndividual>
    


    <!-- http://ontology.library.harvard.edu/geo/EquidistantConic -->

    <owl:NamedIndividual rdf:about="http://ontology.library.harvard.edu/geo/EquidistantConic">
        <projectionPreservationProperty rdf:resource="http://ontology.library.harvard.edu/geo/Equidistant"/>
    </owl:NamedIndividual>
    


    <!-- http://ontology.library.harvard.edu/geo/Equirectangular -->

    <owl:NamedIndividual rdf:about="http://ontology.library.harvard.edu/geo/Equirectangular">
        <projectionPreservationProperty rdf:resource="http://ontology.library.harvard.edu/geo/Equidistant"/>
    </owl:NamedIndividual>
    


    <!-- http://ontology.library.harvard.edu/geo/ExplicitScale -->

    <owl:NamedIndividual rdf:about="http://ontology.library.harvard.edu/geo/ExplicitScale">
        <rdf:type rdf:resource="http://ontology.library.harvard.edu/geo/ScaleAccuracy"/>
        <dcterms:issued>2018-03-26</dcterms:issued>
        <skos:definition xml:lang="en">Scale as stated on the cartographic resource</skos:definition>
        <skos:prefLabel xml:lang="en">Explicit scale</skos:prefLabel>
    </owl:NamedIndividual>
    


    <!-- http://ontology.library.harvard.edu/geo/GNIS -->

    <owl:NamedIndividual rdf:about="http://ontology.library.harvard.edu/geo/GNIS">
        <rdf:type rdf:resource="http://ontology.library.harvard.edu/geo/CartSource"/>
        <dcterms:issued>2018-03-26</dcterms:issued>
        <rdfs:comment xml:lang="en">MARC Cartographic Data Source Code: gnis</rdfs:comment>
        <skos:definition xml:lang="en">Geographic Names Information System (GNIS) (United States Geological Survey, Board on Geographic Names)</skos:definition>
        <skos:prefLabel xml:lang="en">GNIS</skos:prefLabel>
        <foaf:page>https://nhd.usgs.gov/gnis.html</foaf:page>
    </owl:NamedIndividual>
    


    <!-- http://ontology.library.harvard.edu/geo/GNS -->

    <owl:NamedIndividual rdf:about="http://ontology.library.harvard.edu/geo/GNS">
        <rdf:type rdf:resource="http://ontology.library.harvard.edu/geo/CartSource"/>
        <dcterms:issued>2018-03-26</dcterms:issued>
        <rdfs:comment xml:lang="en">MARC Cartographic Data Source Code: geonet</rdfs:comment>
        <skos:definition xml:lang="en">NGA GEOnet Names Server (GNS) (National Geospatial-Intelligence Agency)</skos:definition>
        <skos:prefLabel xml:lang="en">GNS</skos:prefLabel>
        <foaf:page>http://geonames.nga.mil/gns/html/</foaf:page>
    </owl:NamedIndividual>
    


    <!-- http://ontology.library.harvard.edu/geo/Gall -->

    <owl:NamedIndividual rdf:about="http://ontology.library.harvard.edu/geo/Gall">
        <projectionPreservationProperty rdf:resource="http://ontology.library.harvard.edu/geo/Compromise"/>
    </owl:NamedIndividual>
    


    <!-- http://ontology.library.harvard.edu/geo/GallPeters -->

    <owl:NamedIndividual rdf:about="http://ontology.library.harvard.edu/geo/GallPeters">
        <projectionPreservationProperty rdf:resource="http://ontology.library.harvard.edu/geo/EqualArea"/>
    </owl:NamedIndividual>
    


    <!-- http://ontology.library.harvard.edu/geo/GaussKruger -->

    <owl:NamedIndividual rdf:about="http://ontology.library.harvard.edu/geo/GaussKruger">
        <projectionPreservationProperty rdf:resource="http://ontology.library.harvard.edu/geo/Conformal"/>
    </owl:NamedIndividual>
    


    <!-- http://ontology.library.harvard.edu/geo/GeoNames -->

    <owl:NamedIndividual rdf:about="http://ontology.library.harvard.edu/geo/GeoNames">
        <rdf:type rdf:resource="http://ontology.library.harvard.edu/geo/CartSource"/>
        <dcterms:issued>2018-03-26</dcterms:issued>
        <rdfs:comment xml:lang="en">MARC Cartographic Data Source Code: geonames</rdfs:comment>
        <skos:definition xml:lang="en">GeoNames.org geographical database</skos:definition>
        <skos:prefLabel xml:lang="en">GeoNames</skos:prefLabel>
        <foaf:page>http://www.geonames.org/</foaf:page>
    </owl:NamedIndividual>
    


    <!-- http://ontology.library.harvard.edu/geo/GettyTGN -->

    <owl:NamedIndividual rdf:about="http://ontology.library.harvard.edu/geo/GettyTGN">
        <rdf:type rdf:resource="http://ontology.library.harvard.edu/geo/CartSource"/>
        <dcterms:issued>2018-03-26</dcterms:issued>
        <rdfs:comment xml:lang="en">MARC Cartographic Data Source Code: gettytgn</rdfs:comment>
        <skos:definition xml:lang="en">Getty Thesaurus of Geographic Names Online (J. Paul Getty Trust)</skos:definition>
        <skos:prefLabel xml:lang="en">Getty TGN</skos:prefLabel>
        <foaf:page>http://www.getty.edu/research/tools/vocabularies/tgn/index.html</foaf:page>
    </owl:NamedIndividual>
    


    <!-- http://ontology.library.harvard.edu/geo/Gnomonic -->

    <owl:NamedIndividual rdf:about="http://ontology.library.harvard.edu/geo/Gnomonic">
        <rdf:type rdf:resource="http://ontology.library.harvard.edu/geo/ProjectionPreservationProperty"/>
        <projectionPreservationProperty rdf:resource="http://ontology.library.harvard.edu/geo/Gnomonic"/>
    </owl:NamedIndividual>
    


    <!-- http://ontology.library.harvard.edu/geo/GooEarth -->

    <owl:NamedIndividual rdf:about="http://ontology.library.harvard.edu/geo/GooEarth">
        <rdf:type rdf:resource="http://ontology.library.harvard.edu/geo/CartSource"/>
        <dcterms:issued>2018-03-26</dcterms:issued>
        <rdfs:comment xml:lang="en">MARC Cartographic Data Source Code: gooearth</rdfs:comment>
        <skos:definition xml:lang="en">Google Earth</skos:definition>
        <skos:prefLabel xml:lang="en">Google Earth</skos:prefLabel>
        <foaf:page>https://www.google.com/earth/</foaf:page>
    </owl:NamedIndividual>
    


    <!-- http://ontology.library.harvard.edu/geo/GoodesHomolographic -->

    <owl:NamedIndividual rdf:about="http://ontology.library.harvard.edu/geo/GoodesHomolographic">
        <projectionPreservationProperty rdf:resource="http://ontology.library.harvard.edu/geo/EqualArea"/>
    </owl:NamedIndividual>
    


    <!-- http://ontology.library.harvard.edu/geo/GoodesHomolosine -->

    <owl:NamedIndividual rdf:about="http://ontology.library.harvard.edu/geo/GoodesHomolosine">
        <projectionPreservationProperty rdf:resource="http://ontology.library.harvard.edu/geo/EqualArea"/>
    </owl:NamedIndividual>
    


    <!-- http://ontology.library.harvard.edu/geo/InaccurateScale -->

    <owl:NamedIndividual rdf:about="http://ontology.library.harvard.edu/geo/InaccurateScale">
        <rdf:type rdf:resource="http://ontology.library.harvard.edu/geo/ScaleAccuracy"/>
        <dcterms:issued>2018-03-26</dcterms:issued>
        <skos:definition xml:lang="en">Inaccurate scale of cartographic resource</skos:definition>
        <skos:prefLabel xml:lang="en">Inaccurate scale</skos:prefLabel>
    </owl:NamedIndividual>
    


    <!-- http://ontology.library.harvard.edu/geo/Krovak -->

    <owl:NamedIndividual rdf:about="http://ontology.library.harvard.edu/geo/Krovak">
        <projectionPreservationProperty rdf:resource="http://ontology.library.harvard.edu/geo/Conformal"/>
    </owl:NamedIndividual>
    


    <!-- http://ontology.library.harvard.edu/geo/LambertsAzimuthalEqualArea -->

    <owl:NamedIndividual rdf:about="http://ontology.library.harvard.edu/geo/LambertsAzimuthalEqualArea">
        <projectionPreservationProperty rdf:resource="http://ontology.library.harvard.edu/geo/EqualArea"/>
    </owl:NamedIndividual>
    


    <!-- http://ontology.library.harvard.edu/geo/LambertsConformalConic -->

    <owl:NamedIndividual rdf:about="http://ontology.library.harvard.edu/geo/LambertsConformalConic">
        <projectionPreservationProperty rdf:resource="http://ontology.library.harvard.edu/geo/Conformal"/>
    </owl:NamedIndividual>
    


    <!-- http://ontology.library.harvard.edu/geo/LambertsCylindricalEqualArea -->

    <owl:NamedIndividual rdf:about="http://ontology.library.harvard.edu/geo/LambertsCylindricalEqualArea">
        <projectionPreservationProperty rdf:resource="http://ontology.library.harvard.edu/geo/EqualArea"/>
    </owl:NamedIndividual>
    


    <!-- http://ontology.library.harvard.edu/geo/Mercator -->

    <owl:NamedIndividual rdf:about="http://ontology.library.harvard.edu/geo/Mercator">
        <projectionPreservationProperty rdf:resource="http://ontology.library.harvard.edu/geo/Conformal"/>
    </owl:NamedIndividual>
    


    <!-- http://ontology.library.harvard.edu/geo/Miller -->

    <owl:NamedIndividual rdf:about="http://ontology.library.harvard.edu/geo/Miller">
        <projectionPreservationProperty rdf:resource="http://ontology.library.harvard.edu/geo/Compromise"/>
    </owl:NamedIndividual>
    


    <!-- http://ontology.library.harvard.edu/geo/Mollweide -->

    <owl:NamedIndividual rdf:about="http://ontology.library.harvard.edu/geo/Mollweide">
        <projectionPreservationProperty rdf:resource="http://ontology.library.harvard.edu/geo/EqualArea"/>
    </owl:NamedIndividual>
    


    <!-- http://ontology.library.harvard.edu/geo/ObliqueMercator -->

    <owl:NamedIndividual rdf:about="http://ontology.library.harvard.edu/geo/ObliqueMercator">
        <projectionPreservationProperty rdf:resource="http://ontology.library.harvard.edu/geo/Conformal"/>
    </owl:NamedIndividual>
    


    <!-- http://ontology.library.harvard.edu/geo/Orthographic -->

    <owl:NamedIndividual rdf:about="http://ontology.library.harvard.edu/geo/Orthographic">
        <projectionPreservationProperty rdf:resource="http://ontology.library.harvard.edu/geo/Perspective"/>
    </owl:NamedIndividual>
    


    <!-- http://ontology.library.harvard.edu/geo/Perspective -->

    <owl:NamedIndividual rdf:about="http://ontology.library.harvard.edu/geo/Perspective">
        <rdf:type rdf:resource="http://ontology.library.harvard.edu/geo/ProjectionPreservationProperty"/>
        <dcterms:issued>2018-03-26</dcterms:issued>
        <skos:definition xml:lang="en">When the Earth is photographed from space, the camera records the view as a perspective projection. If the camera precisely faces the center of the Earth, the projection is Vertical Perspective. Otherwise, a Tilted Perspective projection is obtained (Wikipedia, General Perspective projection)</skos:definition>
        <skos:prefLabel xml:lang="en">Perspective map projection</skos:prefLabel>
    </owl:NamedIndividual>
    


    <!-- http://ontology.library.harvard.edu/geo/Polyconic -->

    <owl:NamedIndividual rdf:about="http://ontology.library.harvard.edu/geo/Polyconic">
        <projectionPreservationProperty rdf:resource="http://ontology.library.harvard.edu/geo/Compromise"/>
    </owl:NamedIndividual>
    


    <!-- http://ontology.library.harvard.edu/geo/ProjectionEpsg4326 -->

    <owl:NamedIndividual rdf:about="http://ontology.library.harvard.edu/geo/ProjectionEpsg4326">
        <rdf:type rdf:resource="http://id.loc.gov/ontologies/bibframe/Projection"/>
        <bf:identifiedBy rdf:resource="http://ontology.library.harvard.edu/geo/EpsgCode4326"/>
        <dcterms:issued>2018-03-26</dcterms:issued>
        <skos:definition xml:lang="en">World Geodetic System 1984</skos:definition>
        <skos:prefLabel xml:lang="en">WGS 84</skos:prefLabel>
    </owl:NamedIndividual>
    


    <!-- http://ontology.library.harvard.edu/geo/RepresentativeFraction -->

    <owl:NamedIndividual rdf:about="http://ontology.library.harvard.edu/geo/RepresentativeFraction">
        <rdf:type rdf:resource="http://ontology.library.harvard.edu/geo/ScaleSource"/>
        <dcterms:issued>2018-03-26</dcterms:issued>
        <skos:definition xml:lang="en">Source of scale is the representative fraction</skos:definition>
        <skos:prefLabel xml:lang="en">Representative fraction</skos:prefLabel>
    </owl:NamedIndividual>
    


    <!-- http://ontology.library.harvard.edu/geo/Robinson -->

    <owl:NamedIndividual rdf:about="http://ontology.library.harvard.edu/geo/Robinson">
        <projectionPreservationProperty rdf:resource="http://ontology.library.harvard.edu/geo/Compromise"/>
    </owl:NamedIndividual>
    


    <!-- http://ontology.library.harvard.edu/geo/ScaleAccuracyUnknown -->

    <owl:NamedIndividual rdf:about="http://ontology.library.harvard.edu/geo/ScaleAccuracyUnknown">
        <rdf:type rdf:resource="http://ontology.library.harvard.edu/geo/ScaleAccuracy"/>
        <dcterms:issued>2018-03-26</dcterms:issued>
        <skos:definition xml:lang="en">Scale accuracy unknown</skos:definition>
        <skos:prefLabel xml:lang="en">Scale accuracy unknown</skos:prefLabel>
    </owl:NamedIndividual>
    


    <!-- http://ontology.library.harvard.edu/geo/ScaleBar -->

    <owl:NamedIndividual rdf:about="http://ontology.library.harvard.edu/geo/ScaleBar">
        <rdf:type rdf:resource="http://ontology.library.harvard.edu/geo/ScaleSource"/>
        <dcterms:issued>2018-03-26</dcterms:issued>
        <skos:definition xml:lang="en">Source of scale is the scale bar</skos:definition>
        <skos:prefLabel xml:lang="en">Scale bar</skos:prefLabel>
    </owl:NamedIndividual>
    


    <!-- http://ontology.library.harvard.edu/geo/Sinusoidal -->

    <owl:NamedIndividual rdf:about="http://ontology.library.harvard.edu/geo/Sinusoidal">
        <projectionPreservationProperty rdf:resource="http://ontology.library.harvard.edu/geo/EqualArea"/>
        <projectionPreservationProperty rdf:resource="http://ontology.library.harvard.edu/geo/Equidistant"/>
    </owl:NamedIndividual>
    


    <!-- http://ontology.library.harvard.edu/geo/SpaceObliqueMercator -->

    <owl:NamedIndividual rdf:about="http://ontology.library.harvard.edu/geo/SpaceObliqueMercator">
        <projectionPreservationProperty rdf:resource="http://ontology.library.harvard.edu/geo/Conformal"/>
    </owl:NamedIndividual>
    


    <!-- http://ontology.library.harvard.edu/geo/Stereographic -->

    <owl:NamedIndividual rdf:about="http://ontology.library.harvard.edu/geo/Stereographic">
        <projectionPreservationProperty rdf:resource="http://ontology.library.harvard.edu/geo/Conformal"/>
    </owl:NamedIndividual>
    


    <!-- http://ontology.library.harvard.edu/geo/TransverseMercator -->

    <owl:NamedIndividual rdf:about="http://ontology.library.harvard.edu/geo/TransverseMercator">
        <projectionPreservationProperty rdf:resource="http://ontology.library.harvard.edu/geo/Conformal"/>
    </owl:NamedIndividual>
    


    <!-- http://ontology.library.harvard.edu/geo/VanDerGrinten -->

    <owl:NamedIndividual rdf:about="http://ontology.library.harvard.edu/geo/VanDerGrinten">
        <projectionPreservationProperty rdf:resource="http://ontology.library.harvard.edu/geo/Compromise"/>
    </owl:NamedIndividual>
    


    <!-- http://ontology.library.harvard.edu/geo/VerbalStatement -->

    <owl:NamedIndividual rdf:about="http://ontology.library.harvard.edu/geo/VerbalStatement">
        <rdf:type rdf:resource="http://ontology.library.harvard.edu/geo/ScaleSource"/>
        <dcterms:issued>2018-03-26</dcterms:issued>
        <skos:definition xml:lang="en">Source of scale is a verbal statement</skos:definition>
        <skos:prefLabel xml:lang="en">Verbal statement</skos:prefLabel>
    </owl:NamedIndividual>
    


    <!-- http://ontology.library.harvard.edu/geo/Wikiped -->

    <owl:NamedIndividual rdf:about="http://ontology.library.harvard.edu/geo/Wikiped">
        <rdf:type rdf:resource="http://ontology.library.harvard.edu/geo/CartSource"/>
        <dcterms:issued>2018-03-26</dcterms:issued>
        <rdfs:comment xml:lang="en">MARC Cartographic Data Source Code: wikiped</rdfs:comment>
        <skos:definition xml:lang="en">Wikipedia</skos:definition>
        <skos:prefLabel xml:lang="en">Wikipedia</skos:prefLabel>
        <foaf:page>https://www.wikipedia.org/</foaf:page>
    </owl:NamedIndividual>
    


    <!-- 
    ///////////////////////////////////////////////////////////////////////////////////////
    //
    // Annotations
    //
    ///////////////////////////////////////////////////////////////////////////////////////
     -->

    <rdf:Description rdf:about="http://ontology.library.harvard.edu/geo/Aitoff">
        <rdfs:comment xml:lang="en">MARC Map format projection code: aa</rdfs:comment>
        <skos:prefLabel xml:lang="en">Aitoff</skos:prefLabel>
        <skos:prefLabel xml:lang="fr">transformation d’Aitoff appliqué à la projection méridienne de G. Postel</skos:prefLabel>
        <dcterms:issued>2018-03-26</dcterms:issued>
        <rdfs:comment>Type: Pseudoazimuthal</rdfs:comment>
        <skos:definition xml:lang="en">Stretching of modified equatorial azimuthal equidistant map. Boundary is 2:1 ellipse. Largely superseded by Hammer (Wikipedia, List of Map Projections)</skos:definition>
        <skos:prefLabel xml:lang="es">proyección de Aitoff</skos:prefLabel>
        <skos:altfLabel xml:lang="en">Aitoff&apos;s projection</skos:altfLabel>
    </rdf:Description>
    <rdf:Description rdf:about="http://ontology.library.harvard.edu/geo/AlbersEqualArea">
        <skos:altLabel xml:lang="fr">projection d’Albers</skos:altLabel>
        <skos:altLabel xml:lang="en">Albers conic</skos:altLabel>
        <skos:prefLabel xml:lang="fr">projection conique équivalente d&apos;Albers</skos:prefLabel>
        <skos:altLabel xml:lang="fr">tronconique équivalente</skos:altLabel>
        <skos:prefLabel xml:lang="en">Albers equal area</skos:prefLabel>
        <skos:prefLabel xml:lang="es">proyección cónica secante equivalente de Albers</skos:prefLabel>
        <dcterms:issued>2018-03-26</dcterms:issued>
        <rdfs:comment>Type: Conic</rdfs:comment>
        <skos:altLabel xml:lang="en">Albers conical equal-area map projection</skos:altLabel>
        <rdfs:comment xml:lang="en">MARC Map format projection code: ca</rdfs:comment>
        <skos:definition xml:lang="en">Two standard parallels with low distortion between them (Wikipedia, List of Map Projections). The meridians are straight lines that meet in a common point beyond the limits of the map, and the parallels are concentric circles whose center is at the point of intersection of the meridians (Dict. of Mapping)</skos:definition>
    </rdf:Description>
    <rdf:Description rdf:about="http://ontology.library.harvard.edu/geo/Armadillo">
        <rdfs:comment xml:lang="en">MARC Map format projection code: da</rdfs:comment>
        <dcterms:issued>2018-03-26</dcterms:issued>
        <skos:altLabel xml:lang="es">proyección en forma de armadillo</skos:altLabel>
        <skos:definition xml:lang="en">A map projection used for world maps. It is neither conformal nor equal-area but instead affords a view evoking a perspective projection while showing most of the globe instead of the half or less that a perspective would (Wikipedia, Armadillo projection)</skos:definition>
        <rdfs:comment>Type: Other</rdfs:comment>
        <skos:prefLabel xml:lang="en">Armadillo</skos:prefLabel>
    </rdf:Description>
    <rdf:Description rdf:about="http://ontology.library.harvard.edu/geo/AzimuthalEquidistant">
        <skos:altfLabel xml:lang="fr">projection zénithale équidistante</skos:altfLabel>
        <skos:prefLabel xml:lang="en">Azimuthal equidistant</skos:prefLabel>
        <skos:prefLabel xml:lang="es">proyección acimutal equidistante de Postel</skos:prefLabel>
        <skos:altfLabel xml:lang="en">Postel’s projection</skos:altfLabel>
        <rdfs:comment>Type: Azimuthal</rdfs:comment>
        <skos:prefLabel xml:lang="fr">projection de Guillaume Postel</skos:prefLabel>
        <rdfs:comment xml:lang="en">MARC Map format projection code: ae</rdfs:comment>
        <skos:definition xml:lang="en">Distances from centre are conserved. Used as the emblem of the United Nations, extending to 60° S. (Wikipedia, List of Map Projections). Used by the USGS in the National Atlas of the United States of America. Neither equal-area nor conformal (Dict. of Mapping)</skos:definition>
        <dcterms:issued>2018-03-26</dcterms:issued>
    </rdf:Description>
    <rdf:Description rdf:about="http://ontology.library.harvard.edu/geo/Bonne">
        <skos:altLabel xml:lang="fr">projection de la Carte de France</skos:altLabel>
        <skos:altLabel xml:lang="fr">projection dite de Bonne</skos:altLabel>
        <skos:altLabel xml:lang="fr">projection de Flamsteed modifiée</skos:altLabel>
        <skos:definition xml:lang="en">Parallels are equally spaced circular arcs and standard lines. Appearance depends on reference parallel. General case of both Werner and sinusoidal (Wikipedia List of Map Projections)</skos:definition>
        <rdfs:comment xml:lang="en">MARC Map format projection code: cb</rdfs:comment>
        <skos:altLabel xml:lang="fr">projection du Dépôt de la Guerre</skos:altLabel>
        <skos:prefLabel xml:lang="en">Bonne</skos:prefLabel>
        <skos:altLabel xml:lang="en">Bonne’s projection</skos:altLabel>
        <skos:altLabel xml:lang="fr">projection de Bonne</skos:altLabel>
        <dcterms:issued>2018-03-26</dcterms:issued>
        <rdfs:comment>Type: Pseudoconical, cordiform</rdfs:comment>
        <skos:altLabel xml:lang="es">proyección de Bonne</skos:altLabel>
    </rdf:Description>
    <rdf:Description rdf:about="http://ontology.library.harvard.edu/geo/Butterfly">
        <skos:definition xml:lang="en">Projects the globe onto a truncated octahedron with symmetrical components and contiguous land masses that may be displayed in various arrangements (Wikipedia, List of Map Projections)</skos:definition>
        <skos:altLabel xml:lang="en">Cahill&apos;s butterfly map</skos:altLabel>
        <skos:prefLabel xml:lang="en">Butterfly</skos:prefLabel>
        <rdfs:comment xml:lang="en">MARC Map format projection code: db</rdfs:comment>
        <skos:altLabel xml:lang="en">Waterman butterfly projection</skos:altLabel>
        <rdfs:comment>Type: Polyhedral</rdfs:comment>
        <dcterms:issued>2018-03-26</dcterms:issued>
    </rdf:Description>
    <rdf:Description rdf:about="http://ontology.library.harvard.edu/geo/CassiniSoldner">
        <skos:prefLabel xml:lang="es">proyección de Cassini</skos:prefLabel>
        <skos:altfLabel xml:lang="es">proyección de mapas planos</skos:altfLabel>
        <rdfs:comment>Type: Cylindrical</rdfs:comment>
        <skos:prefLabel xml:lang="fr">projection de Cassini</skos:prefLabel>
        <skos:prefLabel xml:lang="en">Cassini-Soldner</skos:prefLabel>
        <skos:altfLabel xml:lang="fr">projection de Soldner</skos:altfLabel>
        <rdfs:comment xml:lang="en">MARC Map format projection code: bl</rdfs:comment>
        <skos:altfLabel xml:lang="fr">projection des cartes plates carrées transverses</skos:altfLabel>
        <skos:altfLabel xml:lang="en">Cassini</skos:altfLabel>
        <skos:definition xml:lang="en">Transverse of equidistant projection; distances along central meridian are conserved. Distances perpendicular to central meridian are preserved (Wikipedia, List of Map Projections)</skos:definition>
        <dcterms:issued>2018-03-26</dcterms:issued>
        <skos:altfLabel xml:lang="fr">coordonnées orthogonales de Hatt</skos:altfLabel>
    </rdf:Description>
    <rdf:Description rdf:about="http://ontology.library.harvard.edu/geo/ConicSpecificTypeUnknown">
        <rdfs:comment xml:lang="en">MARC Map format projection code: cu</rdfs:comment>
        <skos:prefLabel xml:lang="en">Conic, specific type unknown</skos:prefLabel>
        <skos:altLabel xml:lang="en">Tangent conical map projection</skos:altLabel>
        <rdfs:comment>Type: Pseudoconical</rdfs:comment>
        <skos:definition xml:lang="en">Only the projection type (conic) is known, not the specific projection (MARC21). A map projection produced by projecting the geographic meridians and parallels onto a cone which is tangent to (or intersects) the surface of a sphere, and then developing the cone into a plane (Dict. of mapping). In standard presentation, conic (or conical) projections map meridians as straight lines, and parallels as arcs of circles (Wikipedia, List of Map Projections).</skos:definition>
        <dcterms:issued>2018-03-26</dcterms:issued>
    </rdf:Description>
    <rdf:Description rdf:about="http://ontology.library.harvard.edu/geo/Cordiform">
        <skos:definition xml:lang="en">Distances from the North Pole are correct as are the curved distances along parallels and distances along central meridian (Wikipedia, List of Map Projections). Heart-shaped</skos:definition>
        <rdfs:comment xml:lang="en">MARC Map format projection code: dh</rdfs:comment>
        <dcterms:issued>2018-03-26</dcterms:issued>
        <skos:altLabel xml:lang="fr">projection de Werner</skos:altLabel>
        <skos:prefLabel xml:lang="en">Cordiform</skos:prefLabel>
        <skos:altLabel xml:lang="en">Werner’s projection</skos:altLabel>
        <skos:altLabel xml:lang="es">proyección equivalente de Werner</skos:altLabel>
        <rdfs:comment>Type: Pseudoconical</rdfs:comment>
    </rdf:Description>
    <rdf:Description rdf:about="http://ontology.library.harvard.edu/geo/Dimaxion">
        <skos:prefLabel xml:lang="en">Dimaxion</skos:prefLabel>
        <dcterms:issued>2018-03-26</dcterms:issued>
        <rdfs:comment xml:lang="en">MARC Map format projection code: dg</rdfs:comment>
        <skos:altLabel xml:lang="en">Dymaxion projection</skos:altLabel>
        <skos:definition xml:lang="en">The Dymaxion map or Fuller map is a projection of a world map onto the surface of an icosahedron, which can be unfolded and flattened to two dimensions. The flat map is heavily interrupted in order to preserve shapes and sizes. The projection was invented by Buckminster Fuller. The Dymaxion projection is intended only for representations of the entire globe (Wikipedia, Dymaxion map)</skos:definition>
        <rdfs:comment>Type: Polyhedral</rdfs:comment>
        <skos:altLabel xml:lang="es">proyección Dymaxion</skos:altLabel>
        <skos:altLabel xml:lang="en">Dimaxion map</skos:altLabel>
        <skos:altLabel xml:lang="en">Fuller map</skos:altLabel>
    </rdf:Description>
    <rdf:Description rdf:about="http://ontology.library.harvard.edu/geo/Eckert">
        <skos:definition xml:lang="en">Eckert developed six projections. The latitudes are parallel lines in all six projections. The projections come in pairs; in the odd-numbered projections, the latitudes are equally spaced, while their even-numbered counterparts are equal-area.  The three pairs are distinguished by the shapes of the meridians. Eckert I and Eckert II have rectilinear (straight-line) meridians, meeting at the equator at an angle. In Eckert III and Eckert IV, meridians are elliptical, while in Eckert V and Eckert VI, they are sinusoidal (Wikipedia, Eckert projection)</skos:definition>
        <dcterms:issued>2018-03-26</dcterms:issued>
        <rdfs:comment xml:lang="en">MARC Map format projection code: dc</rdfs:comment>
        <rdfs:comment>Type: Pseudocylindrical</rdfs:comment>
        <skos:prefLabel xml:lang="en">Eckert</skos:prefLabel>
    </rdf:Description>
    <rdf:Description rdf:about="http://ontology.library.harvard.edu/geo/EquidistantConic">
        <dcterms:issued>2018-03-26</dcterms:issued>
        <rdfs:comment>Type: Conic</rdfs:comment>
        <rdfs:comment xml:lang="en">MARC Map format projection code: ce</rdfs:comment>
        <skos:definition xml:lang="en">Distances along meridians are conserved, as is distance along one or two standard parallels (Wikipedia, List of Map Projections)</skos:definition>
        <skos:altLabel xml:lang="en">Simple conic</skos:altLabel>
        <skos:prefLabel xml:lang="en">Equidistant conic</skos:prefLabel>
    </rdf:Description>
    <rdf:Description rdf:about="http://ontology.library.harvard.edu/geo/Equirectangular">
        <rdfs:comment xml:lang="en">MARC Map format projection code: bj</rdfs:comment>
        <skos:altfLabel xml:lang="en">Rectangular</skos:altfLabel>
        <skos:prefLabel xml:lang="en">Equirectangular</skos:prefLabel>
        <skos:altfLabel xml:lang="fr">plate carrée</skos:altfLabel>
        <dcterms:issued>2018-03-26</dcterms:issued>
        <rdfs:comment>Type: Cylindrical</rdfs:comment>
        <skos:altfLabel xml:lang="fr">cylindrique équidistante carrée</skos:altfLabel>
        <skos:altfLabel xml:lang="fr">la carte parallélogrammatique</skos:altfLabel>
        <skos:prefLabel xml:lang="fr">projection des cartes plates carrées</skos:prefLabel>
        <skos:altfLabel xml:lang="en">Cylindrical equidistant</skos:altfLabel>
        <skos:altfLabel xml:lang="en">Equidistant cylindrical</skos:altfLabel>
        <skos:definition xml:lang="en">Simplest geometry; distances along meridians are conserved. Plate carrée: special case having the equator as the standard parallel (Wikipedia, List of Map Projections)</skos:definition>
        <skos:prefLabel xml:lang="es">proyección plana cuadrada</skos:prefLabel>
    </rdf:Description>
    <rdf:Description rdf:about="http://ontology.library.harvard.edu/geo/Gall">
        <skos:altfLabel xml:lang="en">Gall stereographic</skos:altfLabel>
        <skos:prefLabel xml:lang="en">Gall</skos:prefLabel>
        <dcterms:issued>2018-03-26</dcterms:issued>
        <rdfs:comment xml:lang="en">MARC Map format projection code: ba</rdfs:comment>
        <skos:definition xml:lang="en">(Similar to Braun). Intended to resemble the Mercator while also displaying the poles. Standard parallels at 45°N/S. Braun is horizontally stretched version with scale correct at equator (Wikipedia, List of Map Projections)</skos:definition>
        <skos:prefLabel xml:lang="es">proyecciones de Gall</skos:prefLabel>
        <rdfs:comment>Type: Cylindrical</rdfs:comment>
    </rdf:Description>
    <rdf:Description rdf:about="http://ontology.library.harvard.edu/geo/GallPeters">
        <rdfs:comment xml:lang="en">Not included in MARC21</rdfs:comment>
        <skos:altfLabel xml:lang="en">Peters</skos:altfLabel>
        <rdfs:comment>Type: Cylindrical</rdfs:comment>
        <skos:definition xml:lang="en">Horizontally compressed version of the Lambert equal-area. Standard parallels at 45°N/S. Aspect ratio of ~1.6. Similar is Balthasart projection with standard parallels at 50°N/S (Wikipedia, List of Map Projections)</skos:definition>
        <skos:prefLabel xml:lang="en">Gall-Peters</skos:prefLabel>
        <skos:altfLabel xml:lang="en">Gall orthographic</skos:altfLabel>
        <dcterms:issued>2018-03-26</dcterms:issued>
    </rdf:Description>
    <rdf:Description rdf:about="http://ontology.library.harvard.edu/geo/GaussKruger">
        <skos:prefLabel xml:lang="fr">projection de Mercator transverse</skos:prefLabel>
        <skos:altfLabel xml:lang="fr">projection de Gauss-Krüger</skos:altfLabel>
        <skos:altfLabel xml:lang="es">proyección de Gauss-Krüger</skos:altfLabel>
        <skos:altfLabel xml:lang="fr">projection de Gauss-Schreiber</skos:altfLabel>
        <skos:prefLabel xml:lang="es">proyección Mercator transversa</skos:prefLabel>
        <owl:sameAs>TransverseMercator</owl:sameAs>
        <skos:altfLabel xml:lang="fr">projection cylindrique conforme de Lambert</skos:altfLabel>
        <skos:definition xml:lang="en">This transverse, ellipsoidal form of the Mercator is finite, unlike the equatorial Mercator. Forms the basis of the Universal Transverse Mercator coordinate system (Wikipedia, List of Map Projections)</skos:definition>
        <dcterms:issued>2018-03-26</dcterms:issued>
        <rdfs:comment xml:lang="en">MARC Map format projection code: bi</rdfs:comment>
        <skos:altfLabel xml:lang="fr">projection de Gauss-Boaga</skos:altfLabel>
        <skos:altfLabel xml:lang="fr">projection de Gauss</skos:altfLabel>
        <rdfs:comment>Type: Cylindrical</rdfs:comment>
        <skos:prefLabel xml:lang="en">Gauss-Kruger</skos:prefLabel>
    </rdf:Description>
    <rdf:Description rdf:about="http://ontology.library.harvard.edu/geo/Gnomonic">
        <skos:definition xml:lang="en">All great circles are straight lines (Wikipedia, List of Map Projections)</skos:definition>
        <skos:prefLabel xml:lang="en">Gnomonic map projection</skos:prefLabel>
        <skos:altfLabel xml:lang="en">Gnomic</skos:altfLabel>
        <skos:prefLabel xml:lang="fr">projection gnomonique</skos:prefLabel>
        <dcterms:issued>2018-03-26</dcterms:issued>
        <rdfs:comment xml:lang="en">MARC Map format projection code: ab</rdfs:comment>
        <skos:prefLabel xml:lang="en">Gnomonic</skos:prefLabel>
        <rdfs:comment>MARC21 uses the term, &quot;Gnomic&quot;</rdfs:comment>
        <skos:definition xml:lang="en">Displays all great circles as straight lines, resulting in any straight line segment on a gnomonic map showing a geodesic, the shortest route between the segment&apos;s two endpoints (Wikipedia, Gnomonic Projection)</skos:definition>
        <skos:prefLabel xml:lang="es">proyección gnomónica</skos:prefLabel>
        <rdfs:comment>Type: Gnomonic</rdfs:comment>
    </rdf:Description>
    <rdf:Description rdf:about="http://ontology.library.harvard.edu/geo/GoodesHomolographic">
        <skos:altfLabel xml:lang="en">Goode&apos;s homalographic</skos:altfLabel>
        <dcterms:issued>2018-03-26</dcterms:issued>
        <skos:altfLabel xml:lang="en">Goode homolosine</skos:altfLabel>
        <skos:prefLabel xml:lang="fr">projection homalographique de Goode</skos:prefLabel>
        <skos:prefLabel xml:lang="en">Goode&apos;s homolographic</skos:prefLabel>
        <rdfs:comment xml:lang="en">MARC Map format projection code: bb</rdfs:comment>
        <rdfs:comment>Type: Pseudocylindrical</rdfs:comment>
        <skos:definition xml:lang="en">Hybrid of Sinusoidal and Mollweide projections. Usually used in interrupted form (Wikipedia, List of Map Projections)</skos:definition>
        <skos:prefLabel xml:lang="es">proyección homalográfica</skos:prefLabel>
    </rdf:Description>
    <rdf:Description rdf:about="http://ontology.library.harvard.edu/geo/GoodesHomolosine">
        <skos:altLabel xml:lang="fr">projection homalographique de Goode</skos:altLabel>
        <rdfs:comment xml:lang="en">MARC Map format projection code: dd</rdfs:comment>
        <skos:altLabel xml:lang="en">Homalographic projection</skos:altLabel>
        <skos:definition xml:lang="en">Hybrid of Sinusoidal and Mollweide projections. Usually used in interrupted form (Wikipedia, List of Map Projections)</skos:definition>
        <skos:altLabel xml:lang="es">proyección homalográfica de Goode</skos:altLabel>
        <rdfs:comment>Type: Pseudocylindrical</rdfs:comment>
        <skos:prefLabel xml:lang="en">Goode&apos;s homolosine</skos:prefLabel>
        <skos:altLabel xml:lang="en">Goode’s homalographic projection</skos:altLabel>
        <dcterms:issued>2018-03-26</dcterms:issued>
    </rdf:Description>
    <rdf:Description rdf:about="http://ontology.library.harvard.edu/geo/Krovak">
        <skos:prefLabel xml:lang="en">Krovak</skos:prefLabel>
        <skos:definition xml:lang="en">The projection is based on Bessel ellipsoid and it was made for the best projection of Czechoslovakia. It is used for State maps of the Czech Republic (Wikipedia, Křovák&apos;s projection)</skos:definition>
        <dcterms:issued>2018-03-26</dcterms:issued>
        <rdfs:comment>Type: Conic</rdfs:comment>
        <skos:altLabel xml:lang="en">Křovák&apos;s projection</skos:altLabel>
        <rdfs:comment xml:lang="en">MARC Map format projection code: bk; classed in MARC21 as a cylindrical projection</rdfs:comment>
    </rdf:Description>
    <rdf:Description rdf:about="http://ontology.library.harvard.edu/geo/LambertsAzimuthalEqualArea">
        <rdfs:comment>Type: Azimuthal</rdfs:comment>
        <skos:altfLabel xml:lang="en">Lambert zenithal equal-area</skos:altfLabel>
        <skos:prefLabel xml:lang="es">proyección acimutal equivalente de Lambert</skos:prefLabel>
        <skos:prefLabel xml:lang="en">Lambert&apos;s azimuthal equal area</skos:prefLabel>
        <skos:altfLabel xml:lang="en">Lambert azimuthal equal-area</skos:altfLabel>
        <skos:prefLabel xml:lang="fr">projection de Lorgna</skos:prefLabel>
        <rdfs:comment xml:lang="en">MARC Map format projection code: ac</rdfs:comment>
        <dcterms:issued>2018-03-26</dcterms:issued>
        <skos:definition xml:lang="en">The straight-line distance between the central point on the map to any other point is the same as the straight-line 3D distance through the globe between the two points (Wikipedia, List of Map Projections)</skos:definition>
        <skos:altfLabel xml:lang="fr">projection azimutale équivalente de Lambert</skos:altfLabel>
    </rdf:Description>
    <rdf:Description rdf:about="http://ontology.library.harvard.edu/geo/LambertsConformalConic">
        <skos:definition xml:lang="en">All geographic meridians are represented by straight lines which meet in a common point outside the limits of the map, and the geographic parallels are represented by a series of arcs of circles having this common point for a center (Dict. of Mapping). Used in aviation charts (Wikipedia, List of Map Projections)</skos:definition>
        <skos:altLabel xml:lang="en">Lambert conformal conic</skos:altLabel>
        <skos:altLabel xml:lang="es">proyección cónica secante conforme de Lambert</skos:altLabel>
        <skos:altLabel xml:lang="es">proyección cónica tangente conforme de Lambert</skos:altLabel>
        <skos:altLabel xml:lang="en">Conformal conical projection with one standard parallel (Lambert)</skos:altLabel>
        <dcterms:issued>2018-03-26</dcterms:issued>
        <rdfs:comment>Type: Conic</rdfs:comment>
        <skos:altLabel xml:lang="fr">projection conique conforme de Lambert (projection à cône tangent)</skos:altLabel>
        <skos:altLabel xml:lang="fr">projection conique conforme de Lambert (projection à cône sécant)</skos:altLabel>
        <skos:altLabel xml:lang="en">Conformal conical projection with two standard parallels (Lambert)</skos:altLabel>
        <skos:prefLabel xml:lang="en">Lambert&apos;s conformal conic</skos:prefLabel>
        <rdfs:comment xml:lang="en">MARC Map format projection code: cc</rdfs:comment>
    </rdf:Description>
    <rdf:Description rdf:about="http://ontology.library.harvard.edu/geo/LambertsCylindricalEqualArea">
        <rdfs:comment xml:lang="en">MARC Map format projection code: bc</rdfs:comment>
        <skos:altfLabel xml:lang="fr">projection isocylindrique</skos:altfLabel>
        <skos:prefLabel xml:lang="es">proyección cilíndrica de Lambert</skos:prefLabel>
        <skos:prefLabel xml:lang="en">Lambert&apos;s cylindrical equal area</skos:prefLabel>
        <rdfs:comment>Type: Cylindrical</rdfs:comment>
        <skos:altfLabel xml:lang="sp">proyección isocilíndrica</skos:altfLabel>
        <skos:altfLabel xml:lang="en">Lambert cylindrical equal area</skos:altfLabel>
        <dcterms:issued>2018-03-26</dcterms:issued>
        <skos:prefLabel xml:lang="fr">projection cylindrique équivalente de Lambert</skos:prefLabel>
        <skos:definition xml:lang="en">Standard parallel at the equator. Aspect ratio of π (3.14). Base projection of the cylindrical equal-area family (Wikipedia, List of Map Projections)</skos:definition>
    </rdf:Description>
    <rdf:Description rdf:about="http://ontology.library.harvard.edu/geo/Mercator">
        <dcterms:issued>2018-03-26</dcterms:issued>
        <skos:definition xml:lang="en">Lines of constant bearing (rhumb lines) are straight, aiding navigation. Areas inflate with latitude, becoming so extreme that the map cannot show the poles (Wikipedia, List of Map Projections). The equator is represented by a straight line true to scale; the geographic meridians are represented by parallel straight lines perpendicular to the line representing the equator; they are spaced according to their distance apart at the equator (Dict. of Mapping)</skos:definition>
        <rdfs:comment>Type: Cylindrical</rdfs:comment>
        <skos:prefLabel xml:lang="es">proyección conforme de Mercator</skos:prefLabel>
        <skos:prefLabel xml:lang="fr">projection de Mercator</skos:prefLabel>
        <skos:altfLabel xml:lang="en">Equatorial cylindrical orthomorphic map projection</skos:altfLabel>
        <skos:prefLabel xml:lang="en">Mercator</skos:prefLabel>
        <rdfs:comment xml:lang="en">MARC Map format projection code: bd</rdfs:comment>
    </rdf:Description>
    <rdf:Description rdf:about="http://ontology.library.harvard.edu/geo/Miller">
        <skos:definition xml:lang="en">Intended to resemble the Mercator while also displaying the poles (Wikipedia, List of Map Projections)</skos:definition>
        <dcterms:issued>2018-03-26</dcterms:issued>
        <skos:prefLabel xml:lang="es">proyecciones cilíndricas de Miller</skos:prefLabel>
        <skos:prefLabel xml:lang="fr">projections cylindriques de Miller</skos:prefLabel>
        <skos:altfLabel xml:lang="en">Miller’s cylindrical projections</skos:altfLabel>
        <rdfs:comment xml:lang="en">MARC Map format projection code: be</rdfs:comment>
        <skos:prefLabel xml:lang="en">Miller</skos:prefLabel>
        <rdfs:comment>Type: Cylindrical</rdfs:comment>
    </rdf:Description>
    <rdf:Description rdf:about="http://ontology.library.harvard.edu/geo/Mollweide">
        <skos:prefLabel xml:lang="en">Mollweide</skos:prefLabel>
        <skos:altfLabel xml:lang="en">Elliptical</skos:altfLabel>
        <skos:altfLabel xml:lang="en">Mollweide homolographic map projection</skos:altfLabel>
        <rdfs:comment xml:lang="en">MARC Map format projection code: bf</rdfs:comment>
        <skos:prefLabel xml:lang="es">proyección de Mollweide</skos:prefLabel>
        <skos:altfLabel xml:lang="en">Homolographic</skos:altfLabel>
        <dcterms:issued>2018-03-26</dcterms:issued>
        <skos:prefLabel xml:lang="fr">projection de Mollweide</skos:prefLabel>
        <rdfs:comment>Type: Pseudocylindrical</rdfs:comment>
        <skos:altfLabel xml:lang="fr">projection homalographique de Babinet</skos:altfLabel>
        <skos:altfLabel xml:lang="en">Babinet</skos:altfLabel>
        <skos:definition xml:lang="en">Meridians are ellipses (Wikipedia, List of Map Projections). Central meridian is represented by a straight line, and the meridian 90 degrees from the center is shown as a full circle (Dict. of Mapping)</skos:definition>
    </rdf:Description>
    <rdf:Description rdf:about="http://ontology.library.harvard.edu/geo/ObliqueMercator">
        <rdfs:comment>Type: Cylindrical</rdfs:comment>
        <skos:altfLabel xml:lang="en">Oblique cylindrical orthomorphic projection</skos:altfLabel>
        <dcterms:issued>2018-03-26</dcterms:issued>
        <skos:definition xml:lang="en">Points on the surface of a sphere or spheroid are conceived as developed by Mercator principles on a cylindrical tangent along an oblique great circle (Wikipedia, List of Map Projections)</skos:definition>
        <rdfs:comment xml:lang="en">MARC Map format projection code: bo</rdfs:comment>
        <skos:prefLabel xml:lang="en">Oblique Mercator</skos:prefLabel>
    </rdf:Description>
    <rdf:Description rdf:about="http://ontology.library.harvard.edu/geo/Orthographic">
        <rdfs:comment>Type: Azimuthal</rdfs:comment>
        <skos:definition xml:lang="en">View from an infinite distance (Wikipedia, List of Map Projections). A perspective azimuthal projection (Dict. of Mapping)</skos:definition>
        <rdfs:comment xml:lang="en">MARC Map format projection code: ad</rdfs:comment>
        <skos:prefLabel xml:lang="es">proyección ortográfica</skos:prefLabel>
        <skos:altfLabel xml:lang="en">Orthogonal map projection</skos:altfLabel>
        <skos:prefLabel xml:lang="fr">projection orthographique</skos:prefLabel>
        <skos:prefLabel xml:lang="en">Orthographic</skos:prefLabel>
        <dcterms:issued>2018-03-26</dcterms:issued>
    </rdf:Description>
    <rdf:Description rdf:about="http://ontology.library.harvard.edu/geo/Polyconic">
        <skos:definition xml:lang="en">A map projection having the central geographic meridian represented by a straight line, along which the spacing for lines representing the geographic parallels is proportional to the distances between the parallels: the parallels are represented by arcs of circles which are not concentric, but whose centers lie on the line representing the central meridian, and whose radii are determined by the lengths of the elements of cones which are tangent along the parallels.  All meridians except the central ones are curved.  The projection is neither conformal nor equal area, but it has been widely used for maps of small areas because of the ease with which it can be constructed (Dict. of mapping)</skos:definition>
        <dcterms:issued>2018-03-26</dcterms:issued>
        <skos:prefLabel xml:lang="en">Polyconic</skos:prefLabel>
        <rdfs:comment xml:lang="en">MARC Map format projection code: cp</rdfs:comment>
        <rdfs:comment>Type: Pseudoconical</rdfs:comment>
    </rdf:Description>
    <rdf:Description rdf:about="http://ontology.library.harvard.edu/geo/Robinson">
        <skos:definition xml:lang="en">Computed by interpolation of tabulated values. Used by Rand McNally since inception and used by NGS 1988–98 (Wikipedia, List of Map Projections)</skos:definition>
        <skos:prefLabel xml:lang="en">Robinson</skos:prefLabel>
        <dcterms:issued>2018-03-26</dcterms:issued>
        <rdfs:comment>Type: Pseudocylindrical</rdfs:comment>
        <rdfs:comment xml:lang="en">MARC Map format projection code: br</rdfs:comment>
    </rdf:Description>
    <rdf:Description rdf:about="http://ontology.library.harvard.edu/geo/Sinusoidal">
        <skos:prefLabel xml:lang="es">proyección sinusoidal de Sanson o de Flamsteed</skos:prefLabel>
        <skos:altfLabel xml:lang="en">Sanson-Flamsteed</skos:altfLabel>
        <skos:prefLabel xml:lang="en">Sinusoidal</skos:prefLabel>
        <rdfs:comment xml:lang="en">MARC Map format projection code: bg</rdfs:comment>
        <skos:altfLabel xml:lang="en">Mercator equal-area</skos:altfLabel>
        <skos:prefLabel xml:lang="fr">projection sinusoïdale de Sanson ou de Flamsteed</skos:prefLabel>
        <dcterms:issued>2018-03-26</dcterms:issued>
        <skos:definition xml:lang="en">Meridians are sinusoids; parallels are equally spaced. Aspect ratio of 2:1. Distances along parallels are conserved (Wikipedia, List of Map Projections)</skos:definition>
        <rdfs:comment>Type: Pseudocylindrical</rdfs:comment>
    </rdf:Description>
    <rdf:Description rdf:about="http://ontology.library.harvard.edu/geo/SpaceObliqueMercator">
        <skos:definition xml:lang="en">The space-oblique Mercator projection provides continual conformal mapping of the swath sensed by a satellite. Scale is true along the ground track, varying 0.01 percent within the normal sensing range of the satellite. Conformality is correct within a few parts per million for the sensing range. Distortion is essentially constant along lines of constant distance parallel to the ground track. SOM is the only projection presented that takes the rotation of Earth into account (Wikipedia, Space-oblique Mercator projection)</skos:definition>
        <dcterms:issued>2018-03-26</dcterms:issued>
        <rdfs:comment xml:lang="en">MARC Map format projection code: bs</rdfs:comment>
        <rdfs:comment>Type: Modified cylindrical</rdfs:comment>
        <skos:prefLabel xml:lang="en">Space oblique Mercator</skos:prefLabel>
    </rdf:Description>
    <rdf:Description rdf:about="http://ontology.library.harvard.edu/geo/Stereographic">
        <skos:prefLabel xml:lang="es">proyección estereográfica</skos:prefLabel>
        <skos:prefLabel xml:lang="fr">projection stéréographique</skos:prefLabel>
        <skos:definition xml:lang="en">Map is infinite in extent with outer hemisphere inflating severely, so it is often used as two hemispheres. Maps all small circles to circles, which is useful for planetary mapping to preserve the shapes of craters (Wikipedia, List of Map Projections)</skos:definition>
        <skos:prefLabel xml:lang="en">Stereographic</skos:prefLabel>
        <rdfs:comment xml:lang="en">MARC Map format projection code: af</rdfs:comment>
        <rdfs:comment>Type: Azimuthal</rdfs:comment>
        <skos:altfLabel xml:lang="en">Azimuthal orthomorphic map projection</skos:altfLabel>
        <dcterms:issued>2018-03-26</dcterms:issued>
    </rdf:Description>
    <rdf:Description rdf:about="http://ontology.library.harvard.edu/geo/TransverseMercator">
        <skos:altfLabel xml:lang="es">proyección de Gauss-Krüger</skos:altfLabel>
        <skos:prefLabel xml:lang="es">proyección Mercator transversa</skos:prefLabel>
        <skos:altfLabel xml:lang="fr">projection de Gauss-Boaga</skos:altfLabel>
        <skos:altfLabel xml:lang="fr">projection cylindrique conforme de Lambert</skos:altfLabel>
        <dcterms:issued>2018-03-26</dcterms:issued>
        <skos:prefLabel xml:lang="fr">projection de Mercator transverse</skos:prefLabel>
        <skos:altfLabel xml:lang="fr">projection de Gauss</skos:altfLabel>
        <rdfs:comment>Type: Cylindrical</rdfs:comment>
        <skos:prefLabel xml:lang="en">Transverse Mercator</skos:prefLabel>
        <owl:sameAs>GaussKruger</owl:sameAs>
        <skos:altfLabel xml:lang="fr">projection de Gauss-Schreiber</skos:altfLabel>
        <skos:altfLabel xml:lang="fr">projection de Gauss-Krüger</skos:altfLabel>
        <skos:definition xml:lang="en">This transverse, ellipsoidal form of the Mercator is finite, unlike the equatorial Mercator. Forms the basis of the Universal Transverse Mercator coordinate system (Wikipedia, List of Map Projections)</skos:definition>
        <rdfs:comment xml:lang="en">MARC Map format projection code: bh</rdfs:comment>
    </rdf:Description>
    <rdf:Description rdf:about="http://ontology.library.harvard.edu/geo/VanDerGrinten">
        <skos:prefLabel xml:lang="en">Van Der Grinten</skos:prefLabel>
        <skos:altLabel xml:lang="es">proyección de Van der Grinten</skos:altLabel>
        <dcterms:issued>2018-03-26</dcterms:issued>
        <skos:definition xml:lang="en">Boundary is a circle. All parallels and meridians are circular arcs. Usually clipped near 80°N/S. Standard world projection of the NGS 1922–88 (Wikipedia, List of Map Projections). Van der Grinten has four projections: I, II, III, and IV</skos:definition>
        <rdfs:comment>Type: Other</rdfs:comment>
        <rdfs:comment xml:lang="en">MARC Map format projection code: df</rdfs:comment>
    </rdf:Description>
</rdf:RDF>



<!-- Generated by the OWL API (version 4.5.9.2019-02-01T07:24:44Z) https://github.com/owlcs/owlapi -->

